WIP: changing the main and alt definitions for subst

Alpha.v
@@ -1,5 +1,5 @@
 
-(** * Alternative definitions of substs and alpha for named formulas *)
+(** * Properties of rename and alpha-equivalence for named formulas *)
 
 (** The NatDed development, Pierre Letouzey, 2019.
     This file is released under the CC0 License, see the LICENSE file *)
@@ -7,249 +7,15 @@
 Require Import Defs NameProofs Nam.
 Import ListNotations.
 Import Nam.Form.
-Import Nam.Form.Alt.
 Local Open Scope bool_scope.
 Local Open Scope lazy_bool_scope.
 Local Open Scope eqb_scope.
 
+Implicit Types x y z v : variable.
+
 Local Coercion Var : variable >-> term.
 
-(** Basic results about [Form.Alt.subst] *)
-
-Ltac simpl_height :=
- match goal with
- | H : S _ < S _ |- _ =>
-   apply Nat.succ_lt_mono in H; simpl_height
- | H : Nat.max _ _ < _ |- _ =>
-   apply Nat.max_lub_lt_iff in H; destruct H; simpl_height
- | _ => idtac
- end.
-
-Lemma hsubst_height v t f h :
-  height f < h ->
-  height (hsubst h v t f) = height f.
-Proof.
- revert v t f.
- induction h.
- - inversion 1.
- - intros v t [ ] LT; simpl in *; simpl_height; auto.
-   case eqb; auto.
-   case negb; simpl; auto.
-   repeat rewrite IHh; auto.
-Qed.
-
-Lemma subst_height v t f :
-  height (subst v t f) = height f.
-Proof.
- apply hsubst_height; auto with *.
-Qed.
-
-Lemma hsubst_indep v t f h h' :
-  height f < h -> height f < h' ->
-  hsubst h v t f = hsubst h' v t f.
-Proof.
- revert h' v t f.
- induction h; [inversion 1|]; destruct h';[inversion 2|].
- destruct f; cbn -[fresh]; intros; simpl_height; f_equal; auto.
- case eqbspec; intros; auto.
- destruct negb eqn:E; f_equal; auto.
- rewrite (IHh h' v0) by auto.
- apply IHh; rewrite hsubst_height; auto.
-Qed.
-
-Lemma hsubst_subst v t f h :
-  height f < h ->
-  hsubst h v t f = subst v t f.
-Proof.
- intros. apply hsubst_indep; auto with *.
-Qed.
-
-Lemma subst_eqn x t f :
- subst x t f =
- match f with
- | True => True
- | False => False
- | Pred p l => Pred p (List.map (Term.subst x t) l)
- | Not f => Not (subst x t f)
- | Op o f f' => Op o (subst x t f) (subst x t f')
- | Quant q v f' =>
-    if x =? v then f
-    else
-      let out_vars := Term.vars t in
-      if negb (Names.mem v out_vars) then
-        Quant q v (subst x t f')
-      else
-        let z := fresh (Names.unions [allvars f; out_vars; Names.singleton x])
-      in
-        Quant q z (subst x t (subst v z f'))
- end.
-Proof.
- destruct f; try reflexivity.
- - unfold subst.
-   set (h1 := S (height f1)).
-   set (h2 := S (height f2)).
-   set (h := height _).
-   assert (LT1 : height f1 < h1) by (cbn; auto with * ).
-   assert (LT2 : height f2 < h2) by (cbn; auto with * ).
-   assert (LT1' : height f1 < h) by (cbn; auto with * ).
-   assert (LT2' : height f2 < h) by (cbn; auto with * ).
-   clearbody h h1 h2.
-   cbn. f_equal; apply hsubst_indep; auto.
- - unfold subst. rewrite hsubst_height; auto with *.
-Qed.
-
-Lemma partialsubst_height x t f :
- height (partialsubst x t f) = height f.
-Proof.
- induction f; cbn; auto. f_equal.
- destruct orb; auto.
-Qed.
-
-Lemma partialsubst_height_lt x t f h :
- height f < h -> height (partialsubst x t f) < h.
-Proof.
- now rewrite partialsubst_height.
-Qed.
-
-Hint Resolve partialsubst_height_lt.
-
-(** Places where [subst] and [partialsubst] will agree *)
-
-Fixpoint IsSimple v t f :=
-  match f with
-  | True | False | Pred _ _ => Logic.True
-  | Not f => IsSimple v t f
-  | Op _ f f' => IsSimple v t f /\ IsSimple v t f'
-  | Quant _ x f => v = x \/ (~Names.In x (Term.vars t)
-                             /\ IsSimple v t f)
-  end.
-
-(** Inductive description of these "simple" substitutions *)
-
-Inductive SimpleSubst (v:variable)(t:term)
- : formula -> formula -> Prop :=
-| SubTr : SimpleSubst v t True True
-| SubFa : SimpleSubst v t False False
-| SubPred p l :
-  SimpleSubst v t (Pred p l) (Pred p (List.map (Term.subst v t) l))
-| SubNot f f' :
-    SimpleSubst v t f f' ->
-    SimpleSubst v t (Not f) (Not f')
-| SubOp o f1 f2 f1' f2' :
-    SimpleSubst v t f1 f1' ->
-    SimpleSubst v t f2 f2' ->
-    SimpleSubst v t (Op o f1 f2) (Op o f1' f2')
-| SubQu1 q f : SimpleSubst v t (Quant q v f) (Quant q v f)
-| SubQu2 q f f' x : x<>v -> ~Names.In x (Term.vars t) ->
-    SimpleSubst v t f f' ->
-    SimpleSubst v t (Quant q x f) (Quant q x f').
-
-Hint Constructors SimpleSubst.
-
-Lemma SimpleSubst_fun v t f f1 f2 :
- SimpleSubst v t f f1 -> SimpleSubst v t f f2 -> f1 = f2.
-Proof.
- intros H1. revert f2.
- induction H1; inversion 1; subst; f_equal; auto; easy.
-Qed.
-
-Lemma SimpleSubst_hsubst x t f h :
-  height f < h ->
-  IsSimple x t f ->
-  SimpleSubst x t f (hsubst h x t f).
-Proof.
- revert f.
- induction h.
- - inversion 1.
- - destruct f; cbn -[fresh];
-   intros Hf IS; simpl_height; auto.
-   + intuition.
-   + case eqbspec.
-     * intros ->; auto.
-     * intros NE.
-       destruct IS as [->|(NI,SI)]; [easy|].
-       rewrite mem_false; cbn; auto.
-Qed.
-
-Lemma SimpleSubst_subst x t f :
-  IsSimple x t f ->
-  SimpleSubst x t f (subst x t f).
-Proof.
- apply SimpleSubst_hsubst. auto with *.
-Qed.
-
-Lemma SimpleSubst_IsSimple x t f f' :
-  SimpleSubst x t f f' -> IsSimple x t f.
-Proof.
- induction 1; cbn; auto.
-Qed.
-
-Lemma SimpleSubst_partialsubst x t f :
-  IsSimple x t f ->
-  SimpleSubst x t f (partialsubst x t f).
-Proof.
- induction f; cbn; auto.
- - intuition.
- - case eqbspec; cbn; intros Hxv IS; subst; auto.
-   destruct IS as [->|(NI,IS)]; [easy|].
-   rewrite mem_false; auto.
-Qed.
-
-Lemma partialsubst_subst x t f :
-  IsSimple x t f -> partialsubst x t f = subst x t f.
-Proof.
- intros IS. apply (SimpleSubst_fun x t f).
- now apply SimpleSubst_partialsubst.
- now apply SimpleSubst_subst.
-Qed.
-
-Lemma SimpleSubst_carac x t f f' :
-  SimpleSubst x t f f' <->
-   partialsubst x t f = f' /\ IsSimple x t f.
-Proof.
-  assert (H := SimpleSubst_partialsubst x t f).
-  split.
-  - intros H'.
-    assert (IS := SimpleSubst_IsSimple x t f f' H').
-    split; auto.
-    apply SimpleSubst_fun with x t f; auto.
-  - intros (<-,IS); auto.
-Qed.
-
-Lemma IsSimple_partialsubst x t v t' f :
-  IsSimple x t f ->
-  IsSimple x t (partialsubst v t' f).
-Proof.
- induction f; cbn; try (intuition; fail).
- intros [->|(NI,IS)]; [now left| right].
- split; auto.
- destruct orb; auto.
-Qed.
-
-(** A sufficient condition for simplicity: *)
-
-Lemma noninter_IsSimple x t f :
-  Names.Empty (Names.inter (allvars f) (Term.vars t)) -> IsSimple x t f.
-Proof.
- induction f; cbn in *; auto.
- intros E; split; (apply IHf1 || apply IHf2); namedec.
- intros E.
- case (eqbspec v x).
- - now left.
- - intros NE. right; split; try apply IHf; namedec.
-Qed.
-
-(** Same, when t is a variable *)
-
-Lemma notin_IsSimple (x z:variable) f :
-  ~Names.In z (allvars f) -> IsSimple x z f.
-Proof.
- intros. apply noninter_IsSimple. cbn. namedec.
-Qed.
-
-Hint Resolve notin_IsSimple.
-
-(** No-op substitutions *)
+(** TERM SUBSTITUTION *)
 
 Lemma term_subst_notin x u t :
  ~Names.In x (Term.vars t) ->
@@ -259,24 +25,6 @@ Proof.
  - case eqbspec; auto. namedec.
  - intros NI. f_equal. apply map_id_iff.
    intros t Ht. apply IH; auto. eapply unionmap_notin; eauto.
-Qed.
-
-Lemma partialsubst_notin x t f :
- ~Names.In x (freevars f) ->
- partialsubst x t f = f.
-Proof.
- induction f; cbn; intros NI; f_equal; auto with set.
- - apply map_id_iff. intros a Ha. apply term_subst_notin.
-   eapply unionmap_notin; eauto.
- - case eqbspec; cbn; auto.
-   intros NE. case Names.mem; f_equal; auto with set.
-Qed.
-
-(** Free variables and substitutions *)
-
-Lemma freevars_allvars f : Names.Subset (freevars f) (allvars f).
-Proof.
- induction f; cbn; auto with set.
 Qed.
 
 Lemma term_vars_subst x u t :
@@ -308,10 +56,9 @@ Proof.
        fold (Term.subst x u t). rewrite (IH t E).
        rewrite (IH' l E'). namedec.
      * intros _.
-       assert (E'' : map (Term.substs [(x, u)]) l = l).
+       assert (E'' : map (Term.subst x u) l = l).
        { apply map_id_iff. intros a Ha.
          apply term_subst_notin. eapply unionmap_notin; eauto. }
-       change Names.elt with variable in *.
        rewrite E''.
        fold (Term.subst x u t). rewrite (IH t E).
        namedec.
@@ -333,115 +80,21 @@ Proof.
    exists a; split; auto. apply H; auto.
 Qed.
 
-Lemma allvars_partialsubst x t f :
- Names.Subset (allvars (partialsubst x t f))
-              (Names.union (allvars f) (Term.vars t)).
-Proof.
- induction f; cbn; try namedec.
- - generalize (term_vars_subst x t (Fun "" l)). cbn. namedec.
- - destruct orb; cbn; namedec.
-Qed.
+(** Combining several term substitutions *)
 
-Lemma allvars_partialsubst_2 x t f :
- IsSimple x t f ->
- Names.In x (freevars f) ->
- Names.Subset (Term.vars t) (allvars (partialsubst x t f)).
-Proof.
- induction f; cbn; intros IS; try namedec.
- - apply (term_vars_subst_in' x t (Fun "" l)).
- - auto.
- - nameiff. destruct IS as (IS1,IS2).
-   intros [IN|IN].
-   rewrite (IHf1 IS1 IN). namedec.
-   rewrite (IHf2 IS2 IN). namedec.
- - case eqbspec; cbn. namedec.
-   nameiff. intros NE (IN,_).
-   destruct IS as [->|(NI,IS)]; [easy|].
-   specialize (IHf IS IN).
-   rewrite mem_false by trivial. cbn. namedec.
-Qed.
-
-Lemma freevars_partialsubst_in x t f :
- IsSimple x t f ->
- Names.In x (freevars f) ->
- Names.Equal (freevars (partialsubst x t f))
-             (Names.union (Names.remove x (freevars f)) (Term.vars t)).
-Proof.
- induction f; cbn; intros IS IN.
- - namedec.
- - namedec.
- - apply (term_vars_subst_in x t (Fun "" l)); auto.
- - auto.
- - destruct IS as (IS1,IS2).
-   rewrite Names.union_spec in IN.
-   destruct (NamesP.In_dec x (freevars f1)) as [IN1|IN1];
-    destruct (NamesP.In_dec x (freevars f2)) as [IN2|IN2];
-    try rewrite (IHf1 IS1 IN1); try rewrite (IHf2 IS2 IN2);
-    try rewrite (partialsubst_notin x t f2) by trivial;
-    try rewrite (partialsubst_notin x t f1) by trivial;
-    namedec.
- - case eqbspec; cbn. namedec.
-   intros. destruct IS as [->|(NI,IS)]; [easy|].
-   rewrite mem_false by trivial.
-   rewrite (IHf IS); namedec.
-Qed.
-
-
-Lemma freevars_partialsubst_subset x t f :
- IsSimple x t f ->
- Names.Subset (freevars (partialsubst x t f))
-              (Names.union (Names.remove x (freevars f)) (Term.vars t)).
-Proof.
- induction f; cbn; intros IS.
- - namedec.
- - namedec.
- - apply (term_vars_subst x t (Fun "" l)).
- - auto.
- - destruct IS as (IS1,IS2).
-   specialize (IHf1 IS1). specialize (IHf2 IS2). namedec.
- - case eqbspec; cbn. namedec.
-   intros. destruct IS as [->|(NI,IS)]; [easy|].
-   specialize (IHf IS).
-   rewrite mem_false by trivial.
-   cbn. namedec.
-Qed.
-
-Lemma freevars_partialsubst_subset2 x t f :
-  IsSimple x t f ->
-  Names.Subset (freevars f)
-               (Names.add x (freevars (partialsubst x t f))).
-Proof.
- intros NE.
- destruct (NamesP.In_dec x (freevars f)).
- - rewrite freevars_partialsubst_in; auto with set.
- - rewrite partialsubst_notin; auto with set.
-Qed.
-
-Lemma freevars_partialsubst_subset3 x t f :
-  IsSimple x t f ->
-  Names.Subset (Names.remove x (freevars f))
-               (freevars (partialsubst x t f)).
-Proof.
- intros NE.
- rewrite (freevars_partialsubst_subset2 x t f); auto with set.
-Qed.
-
-(** Swapping substitutions *)
-
-Lemma term_subst_subst x u y v t :
- x<>y -> ~Names.In x (Term.vars v) ->
-  Term.subst y v (Term.subst x u t) =
-  Term.subst x (Term.subst y v u) (Term.subst y v t).
+Lemma term_subst_subst x u x' u' t :
+ x<>x' -> ~Names.In x (Term.vars u') ->
+  Term.subst x' u' (Term.subst x u t) =
+  Term.subst x (Term.subst x' u' u) (Term.subst x' u' t).
 Proof.
  intros NE NI.
  induction t using term_ind'; cbn.
  - case eqbspec; [intros ->|intros NE'].
-   + change Names.elt with variable in *.
-     rewrite <- eqb_neq in NE. rewrite NE. cbn.
+   + rewrite <- eqb_neq in NE. rewrite NE. cbn.
      now rewrite eqb_refl.
    + case eqbspec; [intros ->|intros NE''].
      * cbn. rewrite eqb_refl.
-       symmetry. now apply term_subst_notin.
+       rewrite term_subst_notin; auto.
      * cbn. rewrite <-eqb_neq in NE',NE''. now rewrite NE', NE''.
  - f_equal.
    rewrite !map_map.
@@ -449,55 +102,225 @@ Proof.
    auto.
 Qed.
 
-Lemma partialsubst_partialsubst x y u v f :
- x<>y -> ~Names.In x (Term.vars v) ->
- IsSimple x u f ->
- IsSimple y v f ->
- partialsubst y v (partialsubst x u f) =
- partialsubst x (Term.subst y v u) (partialsubst y v f).
+Lemma term_subst_chain x y u t :
+ ~Names.In y (Term.vars t) ->
+  Term.subst y u (Term.subst x (Var y) t) = Term.subst x u t.
 Proof.
- intros NE NI.
- induction f; cbn; intros IS1 IS2; f_equal; auto.
+ intros NI.
+ induction t using term_ind'; cbn.
+ - case eqbspec; [intros ->|intros NE].
+   + simpl. now rewrite eqb_refl.
+   + rewrite term_subst_notin; auto with set.
+ - simpl in *. rewrite unionmap_in in NI.
+   f_equal.
+   rewrite !map_map.
+   apply map_ext_in.
+   intros. apply H; auto. contradict NI. now exists a.
+Qed.
+
+Lemma term_subst_bis v z u t :
+ z <> v ->
+ Term.subst v u (Term.subst v (Var z) t) =
+ Term.subst v (Var z) t.
+Proof.
+ induction t as [x | f l IH] using term_ind'; intro H; cbn.
+ - case eqbspec; cbn.
+   + apply eqb_neq in H. now rewrite H.
+   + intros H'. apply eqb_neq in H'. now rewrite H'.
+ - f_equal. rewrite map_map. apply map_ext_iff. intros.
+   apply IH; auto.
+Qed.
+
+(** A fresh "reconciliating" variable could be arbitrary *)
+
+Lemma term_subst_rename x x' z z' t t':
+  ~Names.In z (Names.union (Term.vars t) (Term.vars t')) ->
+  ~Names.In z' (Names.union (Term.vars t) (Term.vars t')) ->
+  Term.subst x z t = Term.subst x' z t' ->
+  Term.subst x z' t = Term.subst x' z' t'.
+Proof.
+ revert t t'.
+ fix IH 1. destruct t, t'; intros Hz Hz'; cbn in *; try easy.
+ - do 2 case eqbspec; intros H H'; subst; intros [=]; namedec.
+ - case eqbspec; intros _ [=].
+ - case eqbspec; intros _ [=].
+ - intros [= <- E]. f_equal. clear f.
+   revert l l0 Hz Hz' E.
+   fix IH' 1. destruct l, l0; intros Hz Hz'; cbn in *; try easy.
+   intros [= E E']. f_equal.
+   + apply IH; auto. namedec. namedec.
+   + apply IH'; auto. namedec. namedec.
+Qed.
+
+(** RENAMING *)
+
+(** For [rename x y f] to be meaningful, we ask for
+    the following precondition. Actually, some simple
+    properties over [rename] may even hold without this
+    precondition. *)
+
+Notation RenOk y f := (~Names.In y (allvars f)).
+
+Lemma rename_height x y f :
+ height (rename x y f) = height f.
+Proof.
+ induction f; cbn; auto. f_equal. destruct eqb; auto.
+Qed.
+
+Lemma rename_height_lt x y f h :
+ height f < h -> height (rename x y f) < h.
+Proof.
+ now rewrite rename_height.
+Qed.
+
+Hint Resolve rename_height_lt.
+
+(** No-op renaming *)
+
+Lemma rename_notin x y f :
+ ~Names.In x (freevars f) ->
+ rename x y f = f.
+Proof.
+ induction f; cbn; intros NI; f_equal; auto with set.
+ - apply map_id_iff. intros a Ha. apply term_subst_notin.
+   eapply unionmap_notin; eauto.
+ - case eqbspec; cbn; auto with set.
+Qed.
+
+(** Free variables and substitutions *)
+
+Lemma freevars_allvars f : Names.Subset (freevars f) (allvars f).
+Proof.
+ induction f; cbn; auto with set.
+Qed.
+
+Lemma allvars_rename x y f :
+ Names.Subset (allvars (rename x y f)) (Names.add y (allvars f)).
+Proof.
+ induction f; cbn; try namedec.
+ - generalize (term_vars_subst x y (Fun "" l)). cbn. namedec.
+ - destruct eqb; cbn; namedec.
+Qed.
+
+Lemma allvars_rename_2 x y f :
+ Names.In x (freevars f) ->
+ Names.In y (allvars (rename x y f)).
+Proof.
+ induction f; cbn; try namedec.
+ - intros. apply (term_vars_subst_in' _ _ (Fun "" l)); auto with set.
+ - case eqbspec; cbn; namedec.
+Qed.
+
+Lemma freevars_rename_in x y f :
+ RenOk y f ->
+ Names.In x (freevars f) ->
+ Names.Equal (freevars (rename x y f))
+             (Names.add y (Names.remove x (freevars f))).
+Proof.
+ induction f; cbn; intros NI IN.
+ - namedec.
+ - namedec.
+ - rewrite (term_vars_subst_in x y (Fun "" l)); simpl; auto with set.
+ - auto.
+ - rewrite Names.union_spec in NI. apply Decidable.not_or in NI.
+   rewrite Names.union_spec in IN.
+   destruct (NamesP.In_dec x (freevars f1)) as [IN1|IN1];
+    destruct (NamesP.In_dec x (freevars f2)) as [IN2|IN2];
+    try rewrite IHf1 by intuition;
+    try rewrite IHf2 by intuition;
+    try rewrite (rename_notin x y f2) by trivial;
+    try rewrite (rename_notin x y f1) by trivial;
+    namedec.
+ - case eqbspec; cbn. namedec.
+   intros. rewrite IHf; namedec.
+Qed.
+
+Lemma freevars_rename_subset x y f :
+ Names.Subset (freevars (rename x y f))
+              (Names.add y (Names.remove x (freevars f))).
+Proof.
+ induction f; cbn.
+ - namedec.
+ - namedec.
+ - rewrite (term_vars_subst x y (Fun "" l)). simpl. namedec.
+ - auto.
+ - rewrite IHf1, IHf2. namedec.
+ - case eqbspec; cbn. namedec.
+   intros. rewrite IHf. namedec.
+Qed.
+
+Lemma freevars_rename_subset2 x y f :
+  Names.Subset (Names.remove x (freevars f))
+               (freevars (rename x y f)).
+Proof.
+ induction f; cbn.
+ - namedec.
+ - namedec.
+ - destruct (NamesP.In_dec x (Term.vars (Fun "" l))) as [H|H]; simpl in *.
+   + rewrite (term_vars_subst_in x y (Fun "" l)); auto. simpl. namedec.
+   + replace (map (Term.subst x y) l) with l. namedec.
+     symmetry. apply map_id_iff.
+     intros. apply term_subst_notin. contradict H.
+     rewrite unionmap_in. now exists a.
+ - auto.
+ - namedec.
+ - case eqbspec; cbn. namedec.
+   intros. rewrite <- IHf. namedec.
+Qed.
+
+Lemma freevars_rename_subset3 x y f :
+  Names.Subset (freevars f)
+               (Names.add x (freevars (rename x y f))).
+Proof.
+ rewrite <- freevars_rename_subset2. namedec.
+Qed.
+
+(** Renaming in chain *)
+
+Lemma rename_chain x y z f :
+ RenOk y f ->
+ rename y z (rename x y f) = rename x z f.
+Proof.
+ induction f; cbn; intros R; f_equal; auto.
+ - rewrite !map_map.
+   apply map_ext_in. intros. apply term_subst_chain.
+   rewrite unionmap_in in R. contradict R. now exists a.
+ - auto with set.
+ - auto with set.
+ - intros. f_equal. repeat case eqbspec; auto.
+   namedec.
+   intros. apply rename_notin. rewrite freevars_allvars. namedec.
+   intros. apply IHf. namedec.
+Qed.
+
+(** Renaming at independent locations *)
+
+Lemma rename_rename x y x' y' f :
+ x<>y -> x<>y' -> x'<>y ->
+ rename y y' (rename x x' f) = rename x x' (rename y y' f).
+Proof.
+ intros XY XY' YX'.
+ induction f; cbn; f_equal; auto.
  - rewrite !map_map.
    apply map_ext. intros.
-   apply term_subst_subst; auto.
+   rewrite term_subst_subst; simpl; auto with set.
+   rewrite <-eqb_neq in YX'. now rewrite YX'.
  - intuition.
- - intuition.
- - repeat (case eqbspec; cbn; auto); intros; subst; try easy.
-   + clear IS2. destruct IS1 as [->|(NI',IS)]; [easy|].
-     rewrite term_subst_notin; auto.
-   + destruct IS1 as [->|(NI1,IS1)]; [easy|].
-     destruct IS2 as [->|(NI2,IS2)]; [easy|].
-     assert (~Names.In v0 (Term.vars (Term.subst y v u))).
-     { rewrite term_vars_subst. namedec. }
-     repeat (rewrite mem_false by trivial).
-     auto.
+Qed.
+
+(** Renaming twice at the same spot *)
+
+Lemma rename_bis v z z' f :
+  z <> v ->
+  rename v z' (rename v z f) = rename v z f.
+Proof.
+ induction f; simpl; intros; f_equal; auto.
+ - rewrite map_map. apply map_ext_iff. intros.
+   apply term_subst_bis; auto.
+ - case eqbspec; simpl; intuition.
 Qed.
 
 (** ALPHA EQUIVALENCE *)
-
-(** An inductive definition, based on [partialsubst].
-    We'll show later that it is equivalent to [Form.AlphaEq]
-    and [Form.Alt.AlphaEq]. *)
-
-Module Ind.
-
-Inductive AlphaEq : formula -> formula -> Prop :=
-| AEqTr : AlphaEq True True
-| AEqFa : AlphaEq False False
-| AEqPred p l : AlphaEq (Pred p l) (Pred p l)
-| AEqNot f f' : AlphaEq f f' -> AlphaEq (Not f) (Not f')
-| AEqOp o f1 f2 f1' f2' :
-  AlphaEq f1 f1' -> AlphaEq f2 f2' ->
-  AlphaEq (Op o f1 f2) (Op o f1' f2')
-| AEqQu q v v' f f' (z:variable) :
-  ~Names.In z (Names.union (allvars f) (allvars f')) ->
-  AlphaEq (partialsubst v z f) (partialsubst v' z f') ->
-  AlphaEq (Quant q v f) (Quant q v' f').
-
-End Ind.
-Import Ind.
-Hint Constructors AlphaEq.
 
 (** A weaker but faster version of namedec *)
 
@@ -511,6 +334,15 @@ Ltac simpl_fresh vars H :=
  rewrite ?Names.add_spec, ?Names.union_spec in H;
  repeat (apply Decidable.not_or in H; destruct H as (?,H));
  clear vars H.
+
+Ltac simpl_height :=
+ match goal with
+ | H : S _ < S _ |- _ =>
+   apply Nat.succ_lt_mono in H; simpl_height
+ | H : Nat.max _ _ < _ |- _ =>
+   apply Nat.max_lub_lt_iff in H; destruct H; simpl_height
+ | _ => idtac
+ end.
 
 Lemma height_ind (P : formula -> Prop) :
  (forall h, (forall f, height f < h -> P f) ->
@@ -550,9 +382,9 @@ Proof.
  revert IHAlphaEq.
  destruct (NamesP.In_dec v (freevars f)) as [E|E];
   destruct (NamesP.In_dec v' (freevars f')) as [E'|E'];
-  try (rewrite (partialsubst_notin v z f E));
-  try (rewrite (partialsubst_notin v' z f' E'));
-  repeat (rewrite freevars_partialsubst_in by auto with set);
+  try (rewrite (rename_notin v z f E));
+  try (rewrite (rename_notin v' z f' E'));
+  repeat (rewrite freevars_rename_in by auto with set);
   cbn;
   rewrite <-!freevars_allvars in H.
  - (* namedec should suffice but take ages ?! *)
@@ -562,87 +394,65 @@ Proof.
  - namedec.
 Qed.
 
-Lemma term_subst_rename (x x' z z' : variable) t t':
-  ~Names.In z (Names.union (Term.vars t) (Term.vars t')) ->
-  ~Names.In z' (Names.union (Term.vars t) (Term.vars t')) ->
-  Term.subst x z t = Term.subst x' z t'  ->
-  Term.subst x z' t = Term.subst x' z' t'.
-Proof.
- revert t t'.
- fix IH 1. destruct t, t'; intros Hz Hz'; cbn in *; try easy.
- - do 2 case eqbspec; intros H H'; subst; intros [=]; namedec.
- - case eqbspec; intros _ [=].
- - case eqbspec; intros _ [=].
- - intros [= <- E]. f_equal. clear f.
-   revert l l0 Hz Hz' E.
-   fix IH' 1. destruct l, l0; intros Hz Hz'; cbn in *; try easy.
-   intros [= E E']. f_equal.
-   + apply IH; auto. namedec. namedec.
-   + apply IH'; auto. namedec. namedec.
-Qed.
-
 (** An adhoc helper lemma for the next one. *)
 
-Lemma AEq_rename_aux f f' (x x' v z z0 : variable) :
+Lemma AEq_rename_aux f f' x x' v z z0 :
   ~Names.In z (Names.union (Names.add x (allvars f))
                          (Names.add v (allvars f'))) ->
   ~Names.In z0 (Names.union (allvars f)
-                          (allvars (partialsubst x' z f'))) ->
-  AlphaEq (partialsubst x z0 f)
-          (partialsubst v z0 (partialsubst x' z f')) ->
+                          (allvars (rename x' z f'))) ->
+  AlphaEq (rename x z0 f) (rename v z0 (rename x' z f')) ->
   ~Names.In x' (freevars f').
 Proof.
  intros Hz Hz0 EQ IN.
- assert (IsSimple x z0 f) by auto with set.
- assert (IsSimple x' z f') by auto with set.
+ assert (RenOk z0 f) by auto with set.
+ assert (RenOk z f') by auto with set.
  assert (z0 <> z).
  { contradict Hz0. subst z0.
    nameiff. right.
    rewrite <- freevars_allvars.
-   rewrite freevars_partialsubst_in; auto. cbn. namedec. }
- assert (NI : ~Names.In z (freevars (partialsubst x z0 f))).
- { rewrite freevars_partialsubst_subset; auto. cbn.
+   rewrite freevars_rename_in; auto. namedec. }
+ assert (NI : ~Names.In z (freevars (rename x z0 f))).
+ { rewrite freevars_rename_subset.
    rewrite freevars_allvars. namedec. }
  apply AEq_freevars in EQ.
  rewrite EQ in NI.
  contradict NI.
- rewrite <- freevars_partialsubst_subset3 by auto with set.
- rewrite freevars_partialsubst_in; auto with set.
+ rewrite <- freevars_rename_subset2.
+ rewrite freevars_rename_in; namedec.
 Qed.
 
 (* The crucial lemma, utterly technical for something so obvious *)
 
-Lemma AEq_rename_any f f' (x x' z z' : variable) :
+Lemma AEq_rename_any f f' x x' z z' :
   ~Names.In z (Names.union (allvars f) (allvars f')) ->
   ~Names.In z' (Names.union (allvars f) (allvars f')) ->
-  AlphaEq (partialsubst x z f) (partialsubst x' z f') ->
-  AlphaEq (partialsubst x z' f) (partialsubst x' z' f').
+  AlphaEq (rename x z f) (rename x' z f') ->
+  AlphaEq (rename x z' f) (rename x' z' f').
 Proof.
  revert f' x x' z z'.
  induction f as [h IH f LT] using height_ind.
  destruct f, f'; intros x x' z z' Hz Hz'; cbn in *; simpl_height;
   try (inversion 1; auto; fail).
  - inversion 1; subst.
-   assert (E : map (Term.subst x z') l =
-                map (Term.subst x' z') l0).
+   assert (E : map (Term.subst x z') l = map (Term.subst x' z') l0).
    { injection (term_subst_rename x x' z z' (Fun "" l) (Fun "" l0)).
      auto. namedec0. namedec0. cbn; f_equal; auto. }
    now rewrite E.
  - inversion 1; eauto.
  - inversion 1; subst; constructor; eapply IH; eauto; namedec0.
- - rewrite !mem_false by namedec0.
-   repeat (case eqbspec; cbn).
+ - repeat (case eqbspec; cbn).
    + trivial.
    + intros NE <-. inversion_clear 1.
      assert (~Names.In x' (freevars f')).
      { eapply AEq_rename_aux; eauto. }
-     rewrite !(partialsubst_notin x') in * by trivial.
+     rewrite !(rename_notin x') in * by trivial.
      apply AEqQu with z0; auto.
    + intros <- NE. inversion_clear 1.
      assert (~Names.In x (freevars f)).
      { apply AEq_sym in H1.
        eapply AEq_rename_aux; eauto; namedec0. }
-     rewrite !(partialsubst_notin x) in * by trivial.
+     rewrite !(rename_notin x) in * by trivial.
      apply AEqQu with z0; auto.
    + intros NE NE'. inversion_clear 1.
 
@@ -651,8 +461,8 @@ Proof.
      set (vars :=
             Names.add x (Names.add x' (Names.add z (Names.add z'
              (Names.unions
-               [ allvars (partialsubst x z f);
-                allvars (partialsubst x' z f');
+               [ allvars (rename x z f);
+                allvars (rename x' z f');
                 allvars f; allvars f']))))).
      destruct (exist_fresh vars) as (z1,Hz1).
      simpl_fresh vars Hz1.
@@ -665,20 +475,16 @@ Proof.
      (* Let's use z1 in the conclusion. *)
 
      apply AEqQu with z1; auto.
-     rewrite !allvars_partialsubst; cbn; namedec0.
+     rewrite !allvars_rename; cbn; namedec0.
      revert H1.
 
      (* We now need to swap the substitutions to
         change z' with z thanks to the IH. *)
 
-     rewrite !(partialsubst_partialsubst x),
-             !(partialsubst_partialsubst x'); auto;
-     rewrite ?term_subst_notin; cbn;
-     rewrite ?Names.singleton_spec; auto;
-     try apply notin_IsSimple; try (namedec0;fail).
-
+     rewrite !(rename_rename x), !(rename_rename x');
+       auto; try (namedec0;fail).
      apply IH; auto;
-     rewrite !allvars_partialsubst; cbn; namedec0.
+     rewrite !allvars_rename; cbn; namedec0.
 Qed.
 
 Lemma AEq_trans f1 f2 f3 :
@@ -701,82 +507,62 @@ Proof.
  split; [exact AEq_refl| exact AEq_sym | exact AEq_trans].
 Qed.
 
-Lemma AEq_partialsubst f f' :
+Lemma AEqQu_iff q v v' f f' z :
+  ~Names.In z (Names.union (allvars f) (allvars f')) ->
+  AlphaEq (Quant q v f) (Quant q v' f') <->
+  AlphaEq (rename v z f) (rename v' z f').
+Proof.
+ intros NI.
+ split.
+ - inversion 1; subst. eapply AEq_rename_any; eauto.
+ - now apply AEqQu.
+Qed.
+
+Lemma AEq_rename f f' :
  AlphaEq f f' ->
- forall x t,
- IsSimple x t f -> IsSimple x t f' ->
- AlphaEq (partialsubst x t f) (partialsubst x t f').
+ forall x y,
+ RenOk y f -> RenOk y f' ->
+ AlphaEq (rename x y f) (rename x y f').
 Proof.
  revert f'.
  induction f as [h IH f LT] using height_ind.
- destruct f, f'; intros EQ x t IS1 IS2; inversion_clear EQ;
+ destruct f, f'; intros EQ x y IS1 IS2; inversion_clear EQ;
   cbn in *; simpl_height; auto.
  - constructor; intuition.
  - rename v0 into v'.
    rename H0 into EQ.
    clear q; rename q0 into q.
-   assert (IsSimple v z f) by auto with set.
-   assert (IsSimple v' z f') by auto with set.
+   assert (RenOk z f) by auto with set.
+   assert (RenOk z f') by auto with set.
    repeat (case eqbspec; cbn); intros; auto.
    + subst v; subst v'.
      apply AEqQu with z; auto.
    + subst v. clear IS1.
-     destruct IS2 as [->|(NI,IS2)]; [easy|].
-     rewrite mem_false by trivial.
-     assert (~Names.In x (freevars f')).
+     rewrite rename_notin; [ apply AEqQu with z; auto | ].
      { case (eqbspec x z).
        - intros ->; rewrite freevars_allvars; namedec.
        - intros NE.
          apply AEq_freevars in EQ.
-         rewrite (freevars_partialsubst_subset2 v' z) by auto.
-         rewrite <- EQ.
-         rewrite freevars_partialsubst_subset by auto.
-         cbn. clear EQ H. namedec. }
-     rewrite partialsubst_notin; auto.
-     apply AEqQu with z; auto.
+         rewrite (freevars_rename_subset3 v' z), <- EQ.
+         rewrite freevars_rename_subset. namedec. }
    + subst v'. clear IS2.
-     destruct IS1 as [->|(NI,IS1)]; [easy|].
-     rewrite mem_false by trivial.
-     assert (~Names.In x (freevars f)).
+     rewrite rename_notin; [ apply AEqQu with z; auto | ].
      { case (eqbspec x z).
        - intros ->; rewrite freevars_allvars; namedec.
        - intros NE.
          apply AEq_freevars in EQ.
-         rewrite (freevars_partialsubst_subset2 v z) by auto.
-         rewrite EQ.
-         rewrite freevars_partialsubst_subset by auto.
-         cbn. clear EQ H. namedec. }
-     rewrite partialsubst_notin; auto.
-     apply AEqQu with z; auto.
-   + destruct IS1 as [->|(NI1,IS1)]; [easy|].
-     destruct IS2 as [->|(NI2,IS2)]; [easy|].
-     rewrite !mem_false by trivial.
-     set (vars :=
-            Names.add x (Names.add v (Names.add v'
-              (Names.unions
-                 [ Term.vars t; allvars f; allvars f'])))).
+         rewrite (freevars_rename_subset3 v z), EQ.
+         rewrite freevars_rename_subset. namedec. }
+   + set (vars :=
+            Names.add x (Names.add v (Names.add v' (Names.add y
+              (Names.unions [allvars f; allvars f']))))).
      destruct (exist_fresh vars) as (z',Hz').
      simpl_fresh vars Hz'.
-     apply AEq_rename_any with (z' := z') in EQ;
-       [ |namedec|namedec].
+     apply AEq_rename_any with (z' := z') in EQ; [ |namedec|namedec].
      clear z H H0 H1.
-     apply AEqQu with z';
-       [rewrite 2 allvars_partialsubst; namedec|].
-     rewrite 2 (partialsubst_partialsubst x); auto;
-     try (rewrite !term_subst_notin by namedec);
-     try (apply IH; auto); cbn; try namedec;
-     try apply IsSimple_partialsubst; auto with set.
-Qed.
-
-Lemma AEq_SimpleSubst f1 f2 f1' f2' x t :
- AlphaEq f1 f2 ->
- SimpleSubst x t f1 f1' -> SimpleSubst x t f2 f2' ->
- AlphaEq f1' f2'.
-Proof.
- intros EQ S1 S2. rewrite SimpleSubst_carac in *.
- destruct S1 as (<-,IS1).
- destruct S2 as (<-,IS2).
- apply AEq_partialsubst; auto.
+     apply AEqQu with z'; [rewrite 2 allvars_rename; namedec|].
+     rewrite 2 (rename_rename x) by auto with set.
+     apply IH; auto; rewrite allvars_rename; namedec.
 Qed.
 
 Lemma AEqQu_nosubst f f' q v :
@@ -786,158 +572,29 @@ Proof.
  set (vars := Names.union (allvars f) (allvars f')).
  destruct (exist_fresh vars) as (z,Hz).
  apply AEqQu with z. exact Hz.
- apply AEq_partialsubst; auto with set.
+ apply AEq_rename; auto with set.
 Qed.
 
-Lemma AEqQu_rename0 f q (v z : variable) :
- IsSimple v z f -> ~Names.In z (freevars f) ->
- AlphaEq (Quant q v f) (Quant q z (partialsubst v z f)).
+Lemma AEqQu_rename f q v z :
+ RenOk z f ->
+ AlphaEq (Quant q v f) (Quant q z (rename v z f)).
 Proof.
- intros IS NI.
+ intros R.
  set (vars := Names.add z (Names.add v (allvars f))).
  destruct (exist_fresh vars) as (z',Hz').
  apply AEqQu with z'.
- - rewrite allvars_partialsubst. cbn. namedec.
+ - rewrite allvars_rename. namedec.
  - case (eqbspec v z).
    + intros ->.
-     rewrite (partialsubst_notin z z); auto. reflexivity.
+     rewrite (rename_notin z z); auto. reflexivity.
+     rewrite freevars_allvars; auto.
    + intros NE.
-     rewrite partialsubst_partialsubst; cbn; auto with set.
-     now rewrite eqb_refl, (partialsubst_notin z).
-Qed.
-
-(** Same, with weaker but clearer precondition *)
-
-Lemma AEqQu_rename f q (v z : variable) :
- ~Names.In z (allvars f) ->
- AlphaEq (Quant q v f) (Quant q z (partialsubst v z f)).
-Proof.
- intros NI. apply AEqQu_rename0; auto with set.
- rewrite freevars_allvars; namedec.
-Qed.
-
-(** The full substitution, first as a relation *)
-
-Definition Subst x t f f' :=
-  exists f0, AlphaEq f f0 /\ SimpleSubst x t f0 f'.
-
-Lemma SimpleSubst_Subst x t f f' :
-  SimpleSubst x t f f' -> Subst x t f f'.
-Proof.
- intros. now exists f.
-Qed.
-
-Lemma Subst_compat x t f1 f2 f1' f2' :
- AlphaEq f1 f2 -> Subst x t f1 f1' -> Subst x t f2 f2' ->
-  AlphaEq f1' f2'.
-Proof.
- intros EQ (f1b & EQ1 & S1) (f2b & EQ2 & S2).
- apply (AEq_SimpleSubst f1b f2b f1' f2' x t); auto.
- transitivity f1. now symmetry.
- transitivity f2; auto.
-Qed.
-
-(* Pseudo constructors for Subst. *)
-
-Lemma Subst_True x t : Subst x t True True.
-Proof.
- now apply SimpleSubst_Subst.
-Qed.
-
-Lemma Subst_False x t : Subst x t False False.
-Proof.
- now apply SimpleSubst_Subst.
-Qed.
-
-Lemma Subst_Pred x t p l :
-  Subst x t (Pred p l) (partialsubst x t (Pred p l)).
-Proof.
- apply SimpleSubst_Subst. now apply SimpleSubst_partialsubst.
-Qed.
-
-Lemma Subst_Not x t f f' :
-  Subst x t f f' -> Subst x t (~f) (~f').
-Proof.
-  intros (f0 & EQ & SI). exists (~ f0)%form; auto.
-Qed.
-
-Lemma Subst_Op x t o f1 f2 f1' f2' :
-  Subst x t f1 f1' -> Subst x t f2 f2' ->
-  Subst x t (Op o f1 f2) (Op o f1' f2').
-Proof.
-  intros (f1b & EQ1 & SI1) (f2b & EQ2 & SI2).
-  exists (Op o f1b f2b); auto.
-Qed.
-
-Lemma Subst_Qu1 x t q f :
-  Subst x t (Quant q x f) (Quant q x f).
-Proof.
-  exists (Quant q x f). split; auto. reflexivity.
-Qed.
-
-Lemma Subst_Qu2 x t q v f f' :
-  x <> v ->
-  ~Names.In v (Term.vars t) ->
-  Subst x t f f' ->
-  Subst x t (Quant q v f) (Quant q v f').
-Proof.
-  intros NE NI (f0 & EQ & IS).
-  exists (Quant q v f0). auto using AEqQu_nosubst.
-Qed.
-
-Lemma Subst_Qu3 x t q (v z : variable) f f' g :
-  x <> v ->
-  ~Names.In z (freevars f) ->
-  Subst v z f f' ->
-  Subst x t (Quant q z f') (Quant q z g) ->
-  Subst x t (Quant q v f) (Quant q z g).
-Proof.
-  intros NE NI (f0 & EQ & SI) (h & EQ' & SI').
-  exists h. split; auto.
-  transitivity (Quant q z f'); auto.
-  transitivity (Quant q v f0).
-  apply AEqQu_nosubst; auto.
-  rewrite SimpleSubst_carac in SI. destruct SI as (<-,IS).
-  apply AEqQu_rename0; auto.
-  apply AEq_freevars in EQ. now rewrite <- EQ.
-Qed.
-
-Lemma Subst_subst x t f : Subst x t f (subst x t f).
-Proof.
- unfold subst.
- set (h := S (height f)).
- assert (LT : height f < h) by (cbn; auto with * ).
- clearbody h. revert x t f LT.
- induction h as [|h IH]; [inversion 1|];
-  intros x t [ ] LT; cbn -[fresh] in *; simpl_height.
- - apply Subst_True.
- - apply Subst_False.
- - apply Subst_Pred.
- - apply Subst_Not; auto.
- - apply Subst_Op; auto.
- - setfresh vars z Hz.
-   case eqbspec.
-   + intros ->. apply Subst_Qu1.
-   + intros NE.
-     destruct (Names.mem v (Term.vars t)) eqn:IN; cbn.
-     * clear IN.
-       apply Subst_Qu3 with (hsubst h v z f); auto.
-       { rewrite freevars_allvars. namedec. }
-       { apply Subst_Qu2; auto; try namedec.
-         apply IH. now rewrite hsubst_height. }
-     * apply Subst_Qu2; auto.
-       rewrite <- Names.mem_spec. now rewrite IN.
-Qed.
-
-Lemma Subst_exists x t f : exists f', Subst x t f f'.
-Proof.
- exists (subst x t f). apply Subst_subst.
+     rewrite rename_chain; auto with set. reflexivity.
 Qed.
 
 Lemma AlphaEq_equiv f f' :
-  Alt.AlphaEq f f' <-> Ind.AlphaEq f f'.
+  αeq f f' = true <-> AlphaEq f f'.
 Proof.
- unfold Alt.AlphaEq.
  unfold αeq.
  set (h := S _).
  assert (LT : height f < h) by (unfold h; auto with *).
@@ -955,36 +612,9 @@ Proof.
    + intros ((<-,?),?); auto.
    + now inversion_clear 1.
  - setfresh vars z Hz.
-   rewrite <- !partialsubst_subst, !lazy_andb_iff, !eqb_eq, IH
-     by auto with set.
+   rewrite !lazy_andb_iff, !eqb_eq, IH by auto with set.
    split.
    + intros (<-,?). apply AEqQu with z; auto with set.
    + inversion_clear 1. split; trivial.
      apply AEq_rename_any with z0; auto. namedec.
-Qed.
-
-Lemma Subst_compat' x t f1 f2 f1' :
- AlphaEq f1 f2 -> Subst x t f1 f1' ->
- exists f2',  Subst x t f2 f2' /\ AlphaEq f1' f2'.
-Proof.
- intros EQ SU.
- exists (subst x t f2).
- split. apply Subst_subst.
- eapply Subst_compat; eauto. apply Subst_subst.
-Qed.
-
-Instance : Proper (eq ==> eq ==> AlphaEq ==> eq ==> iff) Subst.
-Proof.
- intros x x' <- t t' <- f f' Hf g g' <-.
- split.
- - intros (f0 & EQ & SI).
-   exists f0. split; auto. now transitivity f.
- - intros (f0 & EQ & SI).
-   exists f0. split; auto. now transitivity f'.
-Qed.
-
-Instance : Proper (eq ==> eq ==> AlphaEq ==> AlphaEq) subst.
-Proof.
- intros x x' <- t t' <- f f' Hf.
- apply (Subst_compat x t f f'); auto using Subst_subst.
 Qed.
