Equiv.v
@@ -4,7 +4,7 @@
 (** The NatDed development, Pierre Letouzey, 2019.
     This file is released under the CC0 License, see the LICENSE file *)
 
-Require Import Defs NameProofs.
+Require Import Defs NameProofs Alpha.
 Require Nam Mix.
 Import ListNotations.
 Import Nam Nam.Form.
@@ -56,6 +56,30 @@ Fixpoint mix2nam stack f :=
     Nam.Quant q v (mix2nam (v::stack) f)
   end.
 
+(** Simultaneous renamings of many variables.
+    The bindings of this substitution will be handled in parallel,
+    not sequentially. In particular, the variables introduced
+    by a binding aren't modified by other bindings.
+    If the substitution contains several bindings of the same
+    variable, the leftmost binding wins (cf. [list_assoc]). *)
+
+Definition substitution := list (variable * term).
+
+Module Ren.
+
+Definition t := list (variable * variable).
+
+Definition invars (ren : t) :=
+  List.fold_right (fun p vs => Names.add (fst p) vs) Names.empty ren.
+
+Definition outvars (ren : t) :=
+  List.fold_right (fun p vs => Names.add (snd p) vs) Names.empty ren.
+
+Definition vars (ren : t) :=
+  Names.union (invars ren) (outvars ren).
+
+End Ren.
+
 (** First, we prove that [nam2mix] is canonical :
     it sends alpha-equivalent named formulas to equal mixed formulas. *)
 
@@ -63,19 +87,37 @@ Fixpoint mix2nam stack f :=
 
 Module Nam2Mix.
 
-Inductive Inv (vars:Names.t) : Subst.t -> Subst.t -> Prop :=
+Inductive Inv (vars:Names.t) : Ren.t -> Ren.t -> Prop :=
  | InvNil : Inv vars [] []
  | InvCons v v' z sub sub' :
    Inv vars sub sub' ->
    ~Names.In z vars ->
-   ~Names.In z (Nam.Subst.vars sub) ->
-   ~Names.In z (Nam.Subst.vars sub') ->
-   Inv vars ((v,Var z)::sub) ((v',Var z)::sub').
+   ~Names.In z (Ren.vars sub) ->
+   ~Names.In z (Ren.vars sub') ->
+   Inv vars ((v,z)::sub) ((v',z)::sub').
+
+Inductive HalfInv (vars:Names.t) : Ren.t -> Prop :=
+ | HInvNil : HalfInv vars []
+ | HInvCons v z sub :
+   HalfInv vars sub ->
+   ~Names.In z vars ->
+   ~Names.In z (Ren.vars sub) ->
+   HalfInv vars ((v,z)::sub).
 
 End Nam2Mix.
 Import Nam2Mix.
 
-Hint Constructors Inv.
+Hint Constructors Inv HalfInv.
+
+Lemma Inv_HalfInv vars sub sub' : Inv vars sub sub' -> HalfInv vars sub.
+Proof.
+ induction 1; auto.
+Qed.
+
+Lemma Inv_HalfInv' vars sub sub' : Inv vars sub sub' -> HalfInv vars sub'.
+Proof.
+ induction 1; auto.
+Qed.
 
 Lemma Inv_sym vars sub sub' :
  Inv vars sub sub' -> Inv vars sub' sub.
@@ -85,9 +127,9 @@ Qed.
 
 Lemma Inv_notIn sub sub' vars v :
  Inv vars sub sub' ->
-  ~(Names.In v vars /\ Names.In v (Subst.outvars sub)).
+  ~(Names.In v vars /\ Names.In v (Ren.outvars sub)).
 Proof.
- induction 1; unfold Subst.vars in *; simpl; namedec.
+ induction 1; unfold Ren.vars in *; simpl; namedec.
 Qed.
 
 Lemma Inv_weak sub sub' vars vars' :
@@ -96,19 +138,25 @@ Proof.
  induction 2; auto.
 Qed.
 
-Lemma Inv_listassoc_var vars sub sub' :
-  Inv vars sub sub' ->
-  forall v t, list_assoc v sub = Some t -> exists z, t = Var z.
+Lemma HalfInv_weak sub vars vars' :
+  Names.Subset vars' vars -> HalfInv vars sub -> HalfInv vars' sub.
 Proof.
- induction 1.
- - easy.
- - simpl. intros x t.
-   case eqbspec; eauto.
-   intros -> [= <-]. now exists z.
+ induction 2; auto.
+Qed.
+
+Lemma HalfInv_weak' (z:variable) sub vars vars' :
+  Names.Subset vars' (Names.add z vars) ->
+  ~Names.In z (Ren.vars sub) ->
+  HalfInv vars sub -> HalfInv vars' sub.
+Proof.
+ induction 3; auto.
+ constructor; auto.
+ - apply IHHalfInv. unfold Ren.vars in *. simpl in H0. namedec.
+ - rewrite H. unfold Ren.vars in *. simpl in *. namedec.
 Qed.
 
 Lemma list_assoc_some_in v sub z :
-  list_assoc v sub = Some (Var z) -> Names.In z (Subst.outvars sub).
+  list_assoc v sub = Some z -> Names.In z (Ren.outvars sub).
 Proof.
  induction sub as [|(v',t) sub IH]; try easy.
  simpl.
@@ -119,8 +167,8 @@ Qed.
 
 Lemma list_assoc_index vars v v' sub sub' z :
 Inv vars sub sub' ->
-list_assoc v sub = Some (Var z) ->
-list_assoc v' sub' = Some (Var z) ->
+list_assoc v sub = Some z ->
+list_assoc v' sub' = Some z ->
 exists k,
 list_index v (map fst sub) = Some k /\
 list_index v' (map fst sub') = Some k.
@@ -130,9 +178,9 @@ Proof.
  do 2 case eqbspec.
  - intros. now exists 0.
  - intros NE <- [= <-] E. apply list_assoc_some_in in E.
-   unfold Nam.Subst.vars in *. namedec.
+   unfold Ren.vars in *. namedec.
  - intros <- NE E [= <-]. apply list_assoc_some_in in E.
-   unfold Nam.Subst.vars in *. namedec.
+   unfold Ren.vars in *. namedec.
  - intros _ _ E E'. destruct (IHInv E E') as (k & Hk & Hk').
    exists (S k). simpl in *. now rewrite Hk, Hk'.
 Qed.
@@ -141,16 +189,16 @@ Lemma list_index_assoc vars v v' sub sub' n :
 Inv vars sub sub' ->
 list_index v (map fst sub) = Some n ->
 list_index v' (map fst sub') = Some n ->
-exists t,
-list_assoc v sub = Some t /\
-list_assoc v' sub' = Some t.
+exists z,
+list_assoc v sub = Some z /\
+list_assoc v' sub' = Some z.
 Proof.
  intros inv.
  revert n.
  induction inv; try easy.
  simpl.
  do 2 case eqbspec.
- - intros <- <- n [= <-] _. now exists (Nam.Var z).
+ - intros <- <- n [= <-] _. now exists z.
  - intros _ <- n [= <-]. clear IHinv.
    destruct list_index; simpl; congruence.
  - intros <- _ n E [= <-]. clear IHinv.
@@ -163,115 +211,291 @@ Proof.
    destruct (list_index v'); simpl in *; congruence.
 Qed.
 
+Fixpoint foldrename_term sub t :=
+  match sub with
+  | [] => t
+  | (v,z)::sub => foldrename_term sub (Term.subst v (Var z) t)
+  end.
+
+Fixpoint foldrename sub f :=
+  match sub with
+  | [] => f
+  | (v,z)::sub => foldrename sub (rename v z f)
+  end.
+
+Lemma foldrename_True sub : foldrename sub True = True.
+Proof.
+ induction sub as [|(v,z) sub IH]; simpl; auto.
+Qed.
+
+Lemma foldrename_False sub : foldrename sub False = False.
+Proof.
+ induction sub as [|(v,z) sub IH]; simpl; auto.
+Qed.
+
+Lemma foldrename_not sub f :
+ foldrename sub (~f) = (~ foldrename sub f)%form.
+Proof.
+ revert f.
+ induction sub as [|(v,z) sub IH]; simpl; auto.
+Qed.
+
+Lemma foldrename_op sub o f f' :
+ foldrename sub (Op o f f') = Op o (foldrename sub f) (foldrename sub f').
+Proof.
+ revert f f'.
+ induction sub as [|(v,z) sub IH]; simpl; auto.
+Qed.
+
+Lemma foldrename_quant_weak sub q v f :
+ exists f', foldrename sub (Quant q v f) = Quant q v f'.
+Proof.
+ revert f.
+ induction sub as [|(x,z) sub IH]; simpl; auto.
+ intros f. now exists f.
+Qed.
+
+Lemma foldrename_pred sub p l :
+ foldrename sub (Pred p l) = Pred p (List.map (foldrename_term sub) l).
+Proof.
+ revert l.
+ induction sub as [|(x,z) sub IH]; simpl; auto.
+ - intros l. f_equal. symmetry. apply map_id_iff; auto.
+ - intros l. rewrite IH. f_equal. rewrite map_map; auto.
+Qed.
+
+Lemma foldrename_quant_swap sub f q (v:variable) :
+ HalfInv (Names.add v (allvars f)) sub ->
+ AlphaEq (foldrename sub (Quant q v f))
+         (Quant q v (foldrename (list_unassoc v sub) f)).
+Proof.
+ revert f.
+ induction sub as [|(x,t) sub IH].
+ - simpl. reflexivity.
+ - simpl. intros f. inversion 1; subst.
+   case eqbspec; simpl; auto.
+   intros NE.
+   apply IH; auto.
+   eapply HalfInv_weak'; eauto. rewrite allvars_rename. namedec.
+Qed.
+
+Lemma foldrename_rename_swap sub f (v z:variable) :
+ HalfInv (Names.add v (allvars f)) ((v,z)::sub) ->
+ AlphaEq (foldrename sub (rename v z f))
+         (rename v z (foldrename (list_unassoc v sub) f)).
+Proof.
+ revert f.
+ induction sub as [|(x,y) sub IH].
+ - simpl. reflexivity.
+ - simpl. intros f. inversion 1; subst.
+   inversion H3; subst.
+   simpl in H.
+   case eqbspec; simpl.
+   + intros ->.
+     rewrite rename_bis; auto with set.
+     apply IH. constructor; auto.
+     unfold Ren.vars in *. simpl in *; namedec.
+   + intros NE.
+     assert (z <> x).
+     { unfold Ren.vars in *; simpl in *; namedec. }
+     rewrite rename_rename; auto with set.
+     apply IH.
+     apply HalfInv_weak' with y (Names.add v (allvars f)).
+     rewrite allvars_rename; simpl. namedec.
+     unfold Ren.vars in *. simpl in *. namedec.
+     constructor; auto.
+     unfold Ren.vars in *. simpl in *; namedec.
+Qed.
+
+Lemma allvars_foldrename sub f :
+  Names.Subset (allvars (foldrename sub f))
+               (Names.union (Ren.outvars sub) (allvars f)).
+Proof.
+ revert f.
+ induction sub as [|(x,t) sub IH]; simpl; intros.
+ - namedec.
+ - rewrite IH, allvars_rename. namedec.
+Qed.
+
+Lemma unassoc_subset sub v :
+ Names.Subset (Ren.outvars (list_unassoc v sub))
+              (Ren.outvars sub).
+Proof.
+ induction sub as [|(x,y) sub IH]; simpl.
+ - auto with set.
+ - case eqbspec; simpl; auto with set.
+Qed.
+
+Lemma foldrename_term_fun sub f l :
+  foldrename_term sub (Fun f l) = Fun f (map (foldrename_term sub) l).
+Proof.
+ revert f l.
+ induction sub as [|(x,t) sub IH]; cbn; intros.
+ - f_equal. symmetry. apply map_id.
+ - rewrite IH. f_equal. apply map_map.
+Qed.
+
+Lemma foldrename_term_var_id sub (v:variable) :
+  ~ Names.In v (Ren.vars sub) ->
+  foldrename_term sub (Var v) = Var v.
+Proof.
+ revert v.
+ induction sub as [|(x,t) sub IH]; cbn; intros; auto.
+ case eqbspec; auto.
+ - intros <-. namedec.
+ - intros NI. apply IH. unfold Ren.vars. namedec.
+Qed.
+
+Lemma foldrename_term_var sub (v:variable) :
+ HalfInv (Names.singleton v) sub ->
+ foldrename_term sub (Var v) = Var (list_assoc_dft v sub v).
+Proof.
+ revert v.
+ induction sub as [|(x,t) sub IH]; cbn; intros; auto.
+ inversion H; subst.
+ case eqbspec; auto.
+ intros <-. apply foldrename_term_var_id; auto.
+Qed.
+
 Lemma nam2mix_term_ok sub sub' t t' :
  Inv (Names.union (Term.vars t) (Term.vars t')) sub sub' ->
- Term.substs sub t = Term.substs sub' t' <->
- nam2mix_term (map fst sub) t = nam2mix_term (map fst sub') t'.
+ foldrename_term sub t = foldrename_term sub' t' <->
+ nam2mix_term (List.map fst sub) t = nam2mix_term (List.map fst sub') t'.
 Proof.
- revert t t' sub sub'.
- fix IH 1. destruct t as [v|f a], t' as [v'|f' a']; intros sub sub' inv;
-   simpl; rewrite ?list_assoc_dft_alt.
- - simpl in *. split.
-   + destruct (list_assoc v sub) eqn:E, (list_assoc v' sub') eqn:E'.
-     * intros <-.
-       destruct (Inv_listassoc_var _ _ _ inv v t E) as (z, ->).
-       destruct (list_assoc_index _ v v' sub sub' z inv E E') as (k & Hk & Hk').
-       simpl in Hk, Hk'.
-       now rewrite Hk, Hk'.
-     * intros ->.
-       apply list_assoc_some_in in E.
-       destruct (Inv_notIn _ _ _ v' inv). namedec.
-     * intros <-.
-       apply list_assoc_some_in in E'.
-       apply Inv_sym in inv.
-       destruct (Inv_notIn _ _ _ v inv). namedec.
+ revert t t'.
+ fix IH 1. destruct t as [|f l], t' as [|f' l']; cbn; intro IV.
+ - rewrite !foldrename_term_var.
+   2:{ eapply Inv_HalfInv'; eauto. eapply Inv_weak; eauto. namedec. }
+   2:{ eapply Inv_HalfInv; eauto. eapply Inv_weak; eauto. namedec. }
+   rewrite !list_assoc_dft_alt.
+   split.
+   + destruct (list_assoc v sub) as [z|] eqn:EQ;
+     destruct (list_assoc v0 sub') as [z'|] eqn:EQ'.
      * intros [= <-].
-       rewrite list_assoc_index_none in E, E'.
-       simpl in *. now rewrite E, E'.
-   + destruct (list_index v) eqn:E, (list_index v') eqn:E'; intros [= <-].
-     * destruct (list_index_assoc _ _ _ _ _ _ inv E E') as (k & Hk & Hk').
-       simpl in *. now rewrite Hk, Hk'.
-     * rewrite <- list_assoc_index_none in E, E'.
-       simpl in *. now rewrite E,E'.
- - split.
-   + generalize (Inv_listassoc_var _ _ _ inv v).
-     destruct list_assoc as [t|]; try easy.
-     intros E. destruct (E t) as (v', ->); easy.
-   + destruct list_index; easy.
- - split.
-   + apply Inv_sym in inv.
-     generalize (Inv_listassoc_var _ _ _ inv v').
-     destruct list_assoc as [t'|]; try easy.
-     intros E. destruct (E t') as (v, ->); easy.
-   + destruct list_index; easy.
- - split. intros [= <- E]. f_equal.
-   + simpl in inv.
-     clear f. revert a a' E inv.
-     fix IH' 1. destruct a as [|t a], a' as [|t' a']; try easy.
-     simpl.
-     intros [= E E'] inv. f_equal.
-     * apply IH; auto. eapply Inv_weak; eauto. namedec.
-     * apply IH'; auto. eapply Inv_weak; eauto. namedec.
-   + intros [= <- E]. f_equal.
-     simpl in inv.
-     clear f. revert a a' E inv.
-     fix IH' 1. destruct a as [|t a], a' as [|t' a']; try easy.
-     simpl.
-     intros [= E E'] inv. f_equal.
-     * apply IH; auto. eapply Inv_weak; eauto. namedec.
-     * apply IH'; auto. eapply Inv_weak; eauto. namedec.
-Qed.
-
-Lemma term_substs_nil t :
- Term.substs [] t = t.
-Proof.
- induction t using term_ind'; simpl; f_equal; auto.
- apply map_id_iff; auto.
-Qed.
-
-Lemma substs_nil f :
- substs [] f = f.
-Proof.
- induction f; cbn - [fresh]; f_equal; auto.
- apply map_id_iff. intros a _. apply term_substs_nil.
+       destruct (list_assoc_index _ v v0 _ _ z IV) as (n & -> & ->); auto.
+     * intros [=].
+       apply list_assoc_some_in in EQ.
+       apply (Inv_notIn _ _ _ z) in IV. namedec.
+     * intros [=].
+       apply list_assoc_some_in in EQ'.
+       apply Inv_sym in IV.
+       apply (Inv_notIn _ _ _ z') in IV. namedec.
+     * intros [= <-].
+       rewrite list_assoc_index_none in EQ. rewrite EQ.
+       rewrite list_assoc_index_none in EQ'. now rewrite EQ'.
+   + destruct (list_index v (map fst sub)) as [n|] eqn:EQ;
+     destruct (list_index v0 (map fst sub')) as [n'|] eqn:EQ'; try easy.
+     * injection 1 as <-.
+       destruct (list_index_assoc _ v v0 _ _ n IV) as (t & -> & ->); auto.
+     * injection 1 as <-.
+       rewrite <- list_assoc_index_none in EQ. rewrite EQ.
+       rewrite <- list_assoc_index_none in EQ'. now rewrite EQ'.
+ - rewrite foldrename_term_fun.
+   rewrite foldrename_term_var.
+   2:{ eapply Inv_HalfInv; eauto. eapply Inv_weak; eauto. namedec. }
+   destruct list_index; easy.
+ - rewrite foldrename_term_fun.
+   rewrite foldrename_term_var.
+   2:{ eapply Inv_HalfInv'; eauto. eapply Inv_weak; eauto. namedec. }
+   destruct list_index; easy.
+ - rewrite !foldrename_term_fun.
+   assert
+     (map (foldrename_term sub) l = map (foldrename_term sub') l'
+      <-> map (nam2mix_term (map fst sub)) l =
+          map (nam2mix_term (map fst sub')) l').
+   { revert l l' IV.
+     fix IH' 1. destruct l as [|t l], l' as [|t' l']; cbn; intros IV;
+      try easy.
+     split.
+     - injection 1 as EQt EQl. f_equal.
+       + apply IH; auto. eapply Inv_weak; eauto. namedec.
+       + apply IH'; auto. eapply Inv_weak; eauto. namedec.
+     - injection 1 as EQt EQl. f_equal.
+       + apply IH; auto. eapply Inv_weak; eauto. namedec.
+       + apply IH'; auto. eapply Inv_weak; eauto. namedec. }
+   split; injection 1 as <- EQ; f_equal; intuition.
 Qed.
 
 Lemma nam2mix_term_inj t t' :
  nam2mix_term [] t = nam2mix_term [] t' <-> t = t'.
 Proof.
  split; [|now intros ->].
- rewrite <- (nam2mix_term_ok [] []), !term_substs_nil; auto.
+ rewrite <- (nam2mix_term_ok [] []); auto.
 Qed.
 
 Lemma nam2mix_canonical_gen sub sub' f f' :
  Inv (Names.union (allvars f) (allvars f')) sub sub' ->
- αeq_gen sub f sub' f' = true <->
+ AlphaEq (foldrename sub f) (foldrename sub' f') <->
  nam2mix (List.map fst sub) f = nam2mix (List.map fst sub') f'.
 Proof.
  revert f' sub sub'.
- induction f; destruct f'; intros sub sub'; simpl; intros IV; try easy.
- - rewrite lazy_andb_iff, !eqb_eq.
-   assert (H := nam2mix_term_ok sub sub' (Nam.Fun "" l) (Nam.Fun "" l0) IV).
-   simpl.
+ induction f; destruct f'; intros sub sub'; simpl; intros IV;
+  rewrite ?foldrename_True, ?foldrename_False, ?foldrename_not, ?foldrename_op,
+    ?foldrename_pred; try easy;
+  try (destruct (foldrename_quant_weak sub q v f) as (g,->); easy);
+  try (destruct (foldrename_quant_weak sub' q v f') as (g',->); easy).
+ - destruct (nam2mix_term_ok sub sub' (Fun "" l) (Fun "" l0) IV) as (U,V).
+   rewrite !foldrename_term_fun in *. cbn in *.
    split.
-   + intros (<-,E). f_equal. injection (proj1 H); simpl; f_equal; auto.
-   + intros [= <- E]. split; auto. injection (proj2 H); simpl; f_equal; auto.
- - rewrite IHf by auto.
-   split; [intros <- | intros [=]]; easy.
- - rewrite !lazy_andb_iff, !eqb_eq.
-   rewrite IHf1, IHf2 by (eapply Inv_weak; eauto; namedec).
-   split; [intros ((<-,<-),<-)|intros [= <- <- <-]]; easy.
- - rewrite lazy_andb_iff, !eqb_eq.
-   setfresh vars z Hz.
-   rewrite IHf by (constructor; try (eapply Inv_weak; eauto); namedec).
-   simpl.
-   split; [intros (<-,<-) | intros [=]]; easy.
+   + inversion 1; subst. f_equal. injection U; auto. now f_equal.
+   + injection 1 as <- EQ. injection V; auto. now intros ->. now f_equal.
+ - split.
+   + inversion_clear 1. f_equal. apply IHf; auto.
+   + injection 1. rewrite <- IHf; auto.
+ - split.
+   + inversion_clear 1. f_equal.
+     * apply IHf1; auto. eapply Inv_weak; eauto. namedec.
+     * apply IHf2; auto. eapply Inv_weak; eauto. namedec.
+   + injection 1 as <- EQ1 EQ2.
+     rewrite <- IHf1 in EQ1 by (eapply Inv_weak; eauto; namedec).
+     rewrite <- IHf2 in EQ2 by (eapply Inv_weak; eauto; namedec).
+     auto.
+ - destruct (exist_fresh
+               (Names.union
+                  (Names.union (Ren.vars sub) (Ren.vars sub'))
+                  (Names.union (Names.add v (allvars f))
+                               (Names.add v0 (allvars f'))))) as (z,Hz).
+   assert (HalfInv (Names.add v (allvars f)) sub).
+   { eapply Inv_HalfInv; eauto. eapply Inv_weak; eauto. namedec. }
+   assert (HalfInv (Names.add v0 (allvars f')) sub').
+   { eapply Inv_HalfInv'; eauto. eapply Inv_weak; eauto. namedec. }
+   split.
+   + intros EQ.
+     assert (q = q0).
+     { destruct (foldrename_quant_weak sub q v f) as (g,->) in EQ.
+       destruct (foldrename_quant_weak sub' q0 v0 f') as (g',->) in EQ.
+       inversion_clear EQ; auto. }
+     subst q0. f_equal.
+     change (nam2mix (map fst ((v,z)::sub)) f =
+             nam2mix (map fst ((v0,z)::sub')) f').
+     apply IHf.
+     { constructor; auto with set.
+       eapply Inv_weak; eauto. namedec. }
+     { simpl.
+       rewrite !foldrename_rename_swap by (constructor; auto with set).
+       rewrite !foldrename_quant_swap in EQ; auto.
+       apply AEqQu_iff with q; auto.
+       rewrite !allvars_foldrename.
+       rewrite !unassoc_subset. unfold Ren.vars in Hz. namedec. }
+   + injection 1 as <- EQ.
+     change (nam2mix (map fst ((v,z)::sub)) f =
+             nam2mix (map fst ((v0,z)::sub')) f') in EQ.
+     rewrite <- IHf in EQ.
+     2:{ constructor; auto with set.
+         eapply Inv_weak; eauto. namedec. }
+     simpl in EQ.
+     rewrite !foldrename_rename_swap in EQ by (constructor; auto with set).
+     rewrite !foldrename_quant_swap; auto.
+     eapply AEqQu; eauto.
+     rewrite !allvars_foldrename.
+     rewrite !unassoc_subset. unfold Ren.vars in Hz. namedec.
 Qed.
 
 Lemma nam2mix_canonical (f f' : Nam.formula) :
  nam2mix [] f = nam2mix [] f' <-> AlphaEq f f'.
 Proof.
- symmetry. now apply nam2mix_canonical_gen.
+ symmetry.
+ apply (nam2mix_canonical_gen [] []). constructor.
 Qed.
 
 (** Proofs about [mix2nam] *)
@@ -398,19 +622,11 @@ Proof.
  apply nam2mix_bclosed.
 Qed.
 
-Lemma AlphaEq_equivalence :
-  Equivalence AlphaEq.
-Proof.
- constructor.
- - intros f. now apply nam2mix_canonical.
- - intros f f'. rewrite <-!nam2mix_canonical. auto.
- - intros f1 f2 f3. rewrite <-!nam2mix_canonical. apply eq_trans.
-Qed.
-
 Lemma nam2mix_eqb (f f' : Nam.formula) :
  (nam2mix [] f =? nam2mix [] f') = (f =? f').
 Proof.
  case eqbspec; rewrite nam2mix_canonical.
- - apply eq_sym.
- - intros H. symmetry. exact (not_true_is_false _ H).
+ - intros. symmetry. now apply AlphaEq_equiv.
+ - intros H. rewrite <- AlphaEq_equiv in H.
+   symmetry. exact (not_true_is_false _ H).
 Qed.
