AltSubst.v
@@ -1,0 +1,95 @@
+
+(** * An simultaneous definition of substitution for named formulas *)
+
+(** The NatDed development, Pierre Letouzey, 2019.
+    This file is released under the CC0 License, see the LICENSE file *)
+
+Require Import Defs NameProofs Nam Alpha Equiv.
+Import ListNotations.
+Import Nam.Form.
+Local Open Scope bool_scope.
+Local Open Scope lazy_bool_scope.
+Local Open Scope eqb_scope.
+
+Module Subst.
+
+Definition t := substitution.
+
+Definition invars (sub : substitution) :=
+  List.fold_right (fun p vs => Names.add (fst p) vs) Names.empty sub.
+
+Definition outvars (sub : substitution) :=
+  Names.unionmap (fun '(_,t) => Term.vars t) sub.
+
+Definition vars (sub : substitution) :=
+  Names.union (invars sub) (outvars sub).
+
+End Subst.
+
+Module Alt.
+
+(** Term substitution *)
+
+Fixpoint term_substs (sub:substitution) t :=
+  match t with
+  | Var v => list_assoc_dft v sub t
+  | Fun f args => Fun f (List.map (term_substs sub) args)
+  end.
+
+Definition term_subst x u t := term_substs [(x,u)] t.
+
+(** Simultaneous substitution of many variables in a term.
+    Capture of bounded variables is correctly handled. *)
+
+Fixpoint substs (sub : substitution) f :=
+ match f with
+  | True | False => f
+  | Pred p args => Pred p (List.map (term_substs sub) args)
+  | Not f => Not (substs sub f)
+  | Op o f f' => Op o (substs sub f) (substs sub f')
+  | Quant q v f' =>
+    let sub := list_unassoc v sub in
+    let out_vars := Subst.outvars sub in
+    if negb (Names.mem v out_vars) then
+      Quant q v (substs sub f')
+    else
+      (* variable capture : we change v into a fresh variable first *)
+      let z := fresh (Names.unions [allvars f; out_vars; Subst.invars sub])
+      in
+      Quant q z (substs ((v,Var z)::sub) f')
+ end.
+
+(** Substitution of a variable in a term :
+    in [t], [v] is replaced by [u] *)
+
+Definition subst v t f := substs [(v,t)] f.
+
+(** Alpha equivalence *)
+
+Fixpoint αeq_gen sub1 f1 sub2 f2 :=
+  match f1, f2 with
+  | True, True | False, False => true
+  | Pred p1 args1, Pred p2 args2 =>
+     (p1 =? p2) &&&
+      (List.map (term_substs sub1) args1 =?
+       List.map (term_substs sub2) args2)
+  | Not f1, Not f2 => αeq_gen sub1 f1 sub2 f2
+  | Op o1 f1 f1', Op o2 f2 f2' =>
+    (o1 =? o2) &&&
+    αeq_gen sub1 f1 sub2 f2 &&&
+    αeq_gen sub1 f1' sub2 f2'
+  | Quant q1 v1 f1', Quant q2 v2 f2' =>
+    (q1 =? q2) &&&
+    (let z := fresh
+                (Names.unions
+                   [allvars f1; Subst.vars sub1; allvars f2; Subst.vars sub2])
+     in
+     αeq_gen ((v1,Var z)::sub1) f1' ((v2,Var z)::sub2) f2')
+  | _,_ => false
+  end.
+
+Definition αeq f1 f2 := αeq_gen [] f1 [] f2.
+
+Definition AlphaEq f1 f2 := αeq f1 f2 = true.
+
+End Alt.
