Subst.v
@@ -1,0 +1,712 @@
+
+(** * Properties of substitutions for named formulas *)
+
+(** The NatDed development, Pierre Letouzey, 2019.
+    This file is released under the CC0 License, see the LICENSE file *)
+
+Require Import Defs NameProofs Nam Alpha.
+Import ListNotations.
+Import Nam.Form.
+Local Open Scope bool_scope.
+Local Open Scope lazy_bool_scope.
+Local Open Scope eqb_scope.
+
+Implicit Types x y z v : variable.
+
+Local Coercion Var : variable >-> term.
+
+(** Basic results about [Form.subst] *)
+
+Lemma hsubst_height v t f h :
+  height f < h ->
+  height (hsubst h v t f) = height f.
+Proof.
+ revert v t f.
+ induction h.
+ - inversion 1.
+ - intros v t [ ] LT; simpl in *; simpl_height; auto.
+   case eqb; auto.
+   case negb; simpl; auto.
+   rewrite IHh, rename_height; auto.
+Qed.
+
+Lemma subst_height v t f :
+  height (subst v t f) = height f.
+Proof.
+ apply hsubst_height; auto with *.
+Qed.
+
+Lemma hsubst_indep v t f h h' :
+  height f < h -> height f < h' ->
+  hsubst h v t f = hsubst h' v t f.
+Proof.
+ revert h' v t f.
+ induction h; [inversion 1|]; destruct h';[inversion 2|].
+ destruct f; cbn -[fresh]; intros; simpl_height; f_equal; auto.
+ case eqbspec; intros; auto.
+ destruct negb eqn:E; f_equal; auto.
+Qed.
+
+Lemma hsubst_subst v t f h :
+  height f < h ->
+  hsubst h v t f = subst v t f.
+Proof.
+ intros. apply hsubst_indep; auto with *.
+Qed.
+
+(** Places where [subst] and [rename] will agree *)
+
+Lemma rename_subst x y f :
+  RenOk y f -> rename x y f = subst x y f.
+Proof.
+ unfold subst.
+ set (h := S (height f)).
+ assert (LT : height f < h) by (cbn; auto with * ).
+ clearbody h. revert f LT.
+ induction h as [|h IH].
+ - inversion 1.
+ - destruct f; simpl; intros; simpl_height; f_equal; auto with set.
+   case eqbspec; auto.
+   intros NE.
+   rewrite mem_false; simpl; f_equal; auto with set.
+Qed.
+
+Lemma subst_eqn x t f :
+ subst x t f =
+ match f with
+ | True => True
+ | False => False
+ | Pred p l => Pred p (List.map (Term.subst x t) l)
+ | Not f => Not (subst x t f)
+ | Op o f f' => Op o (subst x t f) (subst x t f')
+ | Quant q v f' =>
+    if x =? v then f
+    else
+      let out_vars := Term.vars t in
+      if negb (Names.mem v out_vars) then
+        Quant q v (subst x t f')
+      else
+        let z := fresh (Names.unions [allvars f; out_vars; Names.singleton x])
+      in
+        Quant q z (subst x t (rename v z f'))
+ end.
+Proof.
+ destruct f; try reflexivity.
+ - unfold subst.
+   set (h1 := S (height f1)).
+   set (h2 := S (height f2)).
+   set (h := height _).
+   assert (LT1 : height f1 < h1) by (cbn; auto with * ).
+   assert (LT2 : height f2 < h2) by (cbn; auto with * ).
+   assert (LT1' : height f1 < h) by (cbn; auto with * ).
+   assert (LT2' : height f2 < h) by (cbn; auto with * ).
+   clearbody h h1 h2.
+   cbn. f_equal; apply hsubst_indep; auto.
+ - unfold subst. rewrite rename_height; auto with *.
+Qed.
+
+(** Same, with [subst] instead of [rename] *)
+
+Lemma subst_eqn' x t f :
+ subst x t f =
+ match f with
+ | True => True
+ | False => False
+ | Pred p l => Pred p (List.map (Term.subst x t) l)
+ | Not f => Not (subst x t f)
+ | Op o f f' => Op o (subst x t f) (subst x t f')
+ | Quant q v f' =>
+    if x =? v then f
+    else
+      let out_vars := Term.vars t in
+      if negb (Names.mem v out_vars) then
+        Quant q v (subst x t f')
+      else
+        let z := fresh (Names.unions [allvars f; out_vars; Names.singleton x])
+      in
+        Quant q z (subst x t (subst v (Var z) f'))
+ end.
+Proof.
+ rewrite subst_eqn. destruct f; auto.
+ case eqbspec; auto.
+ intros NE; simpl.
+ destruct (Names.mem v (Term.vars t)) eqn:EQ; simpl; auto.
+ f_equal. f_equal.
+ apply rename_subst.
+ set (vars := Names.union _ _).
+ assert (Hz := fresh_ok vars). namedec.
+Qed.
+
+
+(** A partial substitution, which does *not* handle
+    correctly variable capture (and just return [f] in this case). *)
+
+Fixpoint partialsubst x t f :=
+  match f with
+  | True | False => f
+  | Pred p args => Pred p (List.map (Term.subst x t) args)
+  | Not f => Not (partialsubst x t f)
+  | Op o f f' => Op o (partialsubst x t f) (partialsubst x t f')
+  | Quant q v f' =>
+    Quant q v
+     (if (x=?v) || Names.mem v (Term.vars t) then f'
+      else partialsubst x t f')
+  end.
+
+Lemma partialsubst_height x t f :
+ height (partialsubst x t f) = height f.
+Proof.
+ induction f; cbn; auto. f_equal.
+ destruct orb; auto.
+Qed.
+
+Lemma partialsubst_height_lt x t f h :
+ height f < h -> height (partialsubst x t f) < h.
+Proof.
+ now rewrite partialsubst_height.
+Qed.
+
+Hint Resolve partialsubst_height_lt.
+
+(** Places where [subst] and [partialsubst] will agree *)
+
+Fixpoint IsSimple v t f :=
+  match f with
+  | True | False | Pred _ _ => Logic.True
+  | Not f => IsSimple v t f
+  | Op _ f f' => IsSimple v t f /\ IsSimple v t f'
+  | Quant _ x f => v = x \/ (~Names.In x (Term.vars t)
+                             /\ IsSimple v t f)
+  end.
+
+(** A sufficient condition for simplicity: *)
+
+Lemma noninter_IsSimple x t f :
+  Names.Empty (Names.inter (allvars f) (Term.vars t)) -> IsSimple x t f.
+Proof.
+ induction f; cbn in *; auto.
+ intros E; split; (apply IHf1 || apply IHf2); namedec.
+ intros E.
+ case (eqbspec v x).
+ - now left.
+ - intros NE. right; split; try apply IHf; namedec.
+Qed.
+
+(** Same, when t is a variable *)
+
+Lemma notin_IsSimple (x z:variable) f :
+  ~Names.In z (allvars f) -> IsSimple x z f.
+Proof.
+ intros. apply noninter_IsSimple. cbn. namedec.
+Qed.
+
+Hint Resolve notin_IsSimple.
+
+(** Inductive description of these "simple" substitutions *)
+
+Inductive SimpleSubst (v:variable)(t:term)
+ : formula -> formula -> Prop :=
+| SubTr : SimpleSubst v t True True
+| SubFa : SimpleSubst v t False False
+| SubPred p l :
+  SimpleSubst v t (Pred p l) (Pred p (List.map (Term.subst v t) l))
+| SubNot f f' :
+    SimpleSubst v t f f' ->
+    SimpleSubst v t (Not f) (Not f')
+| SubOp o f1 f2 f1' f2' :
+    SimpleSubst v t f1 f1' ->
+    SimpleSubst v t f2 f2' ->
+    SimpleSubst v t (Op o f1 f2) (Op o f1' f2')
+| SubQu1 q f : SimpleSubst v t (Quant q v f) (Quant q v f)
+| SubQu2 q f f' x : x<>v -> ~Names.In x (Term.vars t) ->
+    SimpleSubst v t f f' ->
+    SimpleSubst v t (Quant q x f) (Quant q x f').
+
+Hint Constructors SimpleSubst.
+
+Lemma SimpleSubst_fun v t f f1 f2 :
+ SimpleSubst v t f f1 -> SimpleSubst v t f f2 -> f1 = f2.
+Proof.
+ intros H1. revert f2.
+ induction H1; inversion 1; subst; f_equal; auto; easy.
+Qed.
+
+Lemma SimpleSubst_hsubst x t f h :
+  height f < h ->
+  IsSimple x t f ->
+  SimpleSubst x t f (hsubst h x t f).
+Proof.
+ revert f.
+ induction h.
+ - inversion 1.
+ - destruct f; cbn -[fresh];
+   intros Hf IS; simpl_height; auto.
+   + intuition.
+   + case eqbspec.
+     * intros ->; auto.
+     * intros NE.
+       destruct IS as [->|(NI,SI)]; [easy|].
+       rewrite mem_false; cbn; auto.
+Qed.
+
+Lemma SimpleSubst_subst x t f :
+  IsSimple x t f ->
+  SimpleSubst x t f (subst x t f).
+Proof.
+ apply SimpleSubst_hsubst. auto with *.
+Qed.
+
+Lemma SimpleSubst_IsSimple x t f f' :
+  SimpleSubst x t f f' -> IsSimple x t f.
+Proof.
+ induction 1; cbn; auto.
+Qed.
+
+Lemma SimpleSubst_partialsubst x t f :
+  IsSimple x t f ->
+  SimpleSubst x t f (partialsubst x t f).
+Proof.
+ induction f; cbn; auto.
+ - intuition.
+ - case eqbspec; cbn; intros Hxv IS; subst; auto.
+   destruct IS as [->|(NI,IS)]; [easy|].
+   rewrite mem_false; auto.
+Qed.
+
+Lemma rename_partialsubst x y f :
+ RenOk y f ->
+ rename x y f = partialsubst x (Var y) f.
+Proof.
+ induction f; cbn; intros; f_equal; auto with set.
+ case eqbspec; simpl; auto.
+ rewrite mem_false; auto with set.
+Qed.
+
+Lemma partialsubst_subst x t f :
+  IsSimple x t f -> partialsubst x t f = subst x t f.
+Proof.
+ intros IS. apply (SimpleSubst_fun x t f).
+ now apply SimpleSubst_partialsubst.
+ now apply SimpleSubst_subst.
+Qed.
+
+Lemma SimpleSubst_carac x t f f' :
+  SimpleSubst x t f f' <->
+   partialsubst x t f = f' /\ IsSimple x t f.
+Proof.
+  assert (H := SimpleSubst_partialsubst x t f).
+  split.
+  - intros H'.
+    assert (IS := SimpleSubst_IsSimple x t f f' H').
+    split; auto.
+    apply SimpleSubst_fun with x t f; auto.
+  - intros (<-,IS); auto.
+Qed.
+
+Lemma IsSimple_partialsubst x t v t' f :
+  IsSimple x t f ->
+  IsSimple x t (partialsubst v t' f).
+Proof.
+ induction f; cbn; try (intuition; fail).
+ intros [->|(NI,IS)]; [now left| right].
+ split; auto.
+ destruct orb; auto.
+Qed.
+
+(** No-op substitutions *)
+
+Lemma partialsubst_notin x t f :
+ ~Names.In x (freevars f) ->
+ partialsubst x t f = f.
+Proof.
+ induction f; cbn; intros NI; f_equal; auto with set.
+ - apply map_id_iff. intros a Ha. apply term_subst_notin.
+   eapply unionmap_notin; eauto.
+ - case eqbspec; cbn; auto.
+   intros NE. case Names.mem; f_equal; auto with set.
+Qed.
+
+(** Free variables and substitutions *)
+
+Lemma allvars_partialsubst x t f :
+ Names.Subset (allvars (partialsubst x t f))
+              (Names.union (allvars f) (Term.vars t)).
+Proof.
+ induction f; cbn; try namedec.
+ - generalize (term_vars_subst x t (Fun "" l)). cbn. namedec.
+ - destruct orb; cbn; namedec.
+Qed.
+
+Lemma allvars_partialsubst_2 x t f :
+ IsSimple x t f ->
+ Names.In x (freevars f) ->
+ Names.Subset (Term.vars t) (allvars (partialsubst x t f)).
+Proof.
+ induction f; cbn; intros IS; try namedec.
+ - apply (term_vars_subst_in' x t (Fun "" l)).
+ - auto.
+ - nameiff. destruct IS as (IS1,IS2).
+   intros [IN|IN].
+   rewrite (IHf1 IS1 IN). namedec.
+   rewrite (IHf2 IS2 IN). namedec.
+ - case eqbspec; cbn. namedec.
+   nameiff. intros NE (IN,_).
+   destruct IS as [->|(NI,IS)]; [easy|].
+   specialize (IHf IS IN).
+   rewrite mem_false by trivial. cbn. namedec.
+Qed.
+
+Lemma freevars_partialsubst_in x t f :
+ IsSimple x t f ->
+ Names.In x (freevars f) ->
+ Names.Equal (freevars (partialsubst x t f))
+             (Names.union (Names.remove x (freevars f)) (Term.vars t)).
+Proof.
+ induction f; cbn; intros IS IN.
+ - namedec.
+ - namedec.
+ - apply (term_vars_subst_in x t (Fun "" l)); auto.
+ - auto.
+ - destruct IS as (IS1,IS2).
+   rewrite Names.union_spec in IN.
+   destruct (NamesP.In_dec x (freevars f1)) as [IN1|IN1];
+    destruct (NamesP.In_dec x (freevars f2)) as [IN2|IN2];
+    try rewrite (IHf1 IS1 IN1); try rewrite (IHf2 IS2 IN2);
+    try rewrite (partialsubst_notin x t f2) by trivial;
+    try rewrite (partialsubst_notin x t f1) by trivial;
+    namedec.
+ - case eqbspec; cbn. namedec.
+   intros. destruct IS as [->|(NI,IS)]; [easy|].
+   rewrite mem_false by trivial.
+   rewrite (IHf IS); namedec.
+Qed.
+
+
+Lemma freevars_partialsubst_subset x t f :
+ IsSimple x t f ->
+ Names.Subset (freevars (partialsubst x t f))
+              (Names.union (Names.remove x (freevars f)) (Term.vars t)).
+Proof.
+ induction f; cbn; intros IS.
+ - namedec.
+ - namedec.
+ - apply (term_vars_subst x t (Fun "" l)).
+ - auto.
+ - destruct IS as (IS1,IS2).
+   specialize (IHf1 IS1). specialize (IHf2 IS2). namedec.
+ - case eqbspec; cbn. namedec.
+   intros. destruct IS as [->|(NI,IS)]; [easy|].
+   specialize (IHf IS).
+   rewrite mem_false by trivial.
+   cbn. namedec.
+Qed.
+
+Lemma freevars_partialsubst_subset2 x t f :
+  IsSimple x t f ->
+  Names.Subset (freevars f)
+               (Names.add x (freevars (partialsubst x t f))).
+Proof.
+ intros NE.
+ destruct (NamesP.In_dec x (freevars f)).
+ - rewrite freevars_partialsubst_in; auto with set.
+ - rewrite partialsubst_notin; auto with set.
+Qed.
+
+Lemma freevars_partialsubst_subset3 x t f :
+  IsSimple x t f ->
+  Names.Subset (Names.remove x (freevars f))
+               (freevars (partialsubst x t f)).
+Proof.
+ intros NE.
+ rewrite (freevars_partialsubst_subset2 x t f); auto with set.
+Qed.
+
+(** Swapping substitutions *)
+
+Lemma partialsubst_partialsubst x x' u u' f :
+ x<>x' -> ~Names.In x (Term.vars u') ->
+ IsSimple x u f ->
+ IsSimple x' u' f ->
+ partialsubst x' u' (partialsubst x u f) =
+ partialsubst x (Term.subst x' u' u) (partialsubst x' u' f).
+Proof.
+ intros NE NI.
+ induction f; cbn; intros IS1 IS2; f_equal; auto.
+ - rewrite !map_map.
+   apply map_ext. intros.
+   apply term_subst_subst; auto.
+ - intuition.
+ - intuition.
+ - repeat (case eqbspec; cbn; auto); intros; subst; try easy.
+   + clear IS2. destruct IS1 as [->|(NI',IS)]; [easy|].
+     rewrite term_subst_notin; auto.
+   + destruct IS1 as [->|(NI1,IS1)]; [easy|].
+     destruct IS2 as [->|(NI2,IS2)]; [easy|].
+     assert (~Names.In v (Term.vars (Term.subst x' u' u))).
+     { rewrite term_vars_subst. namedec. }
+     repeat (rewrite mem_false by trivial).
+     auto.
+Qed.
+
+(** When defined, [partialsubst] is compatible with alpha-equivalence *)
+
+Lemma AEq_partialsubst f f' :
+ AlphaEq f f' ->
+ forall x t,
+ IsSimple x t f -> IsSimple x t f' ->
+ AlphaEq (partialsubst x t f) (partialsubst x t f').
+Proof.
+ revert f'.
+ induction f as [h IH f LT] using height_ind.
+ destruct f, f'; intros EQ x t IS1 IS2; inversion_clear EQ;
+  cbn in *; simpl_height; auto.
+ - constructor; intuition.
+ - rename v0 into v'.
+   rename H0 into EQ.
+   clear q; rename q0 into q.
+   assert (IsSimple v z f) by auto with set.
+   assert (IsSimple v' z f') by auto with set.
+   repeat (case eqbspec; cbn); intros; auto.
+   + subst v; subst v'.
+     apply AEqQu with z; auto.
+   + subst v. clear IS1.
+     destruct IS2 as [->|(NI,IS2)]; [easy|].
+     rewrite mem_false by trivial.
+     rewrite partialsubst_notin. apply AEqQu with z; auto.
+     { case (eqbspec x z).
+       - intros ->; rewrite freevars_allvars; namedec.
+       - intros NE.
+         apply AEq_freevars in EQ.
+         rewrite (freevars_rename_subset3 v' z), <- EQ.
+         rewrite freevars_rename_subset. namedec. }
+   + subst v'. clear IS2.
+     destruct IS1 as [->|(NI,IS1)]; [easy|].
+     rewrite mem_false by trivial.
+     rewrite partialsubst_notin. apply AEqQu with z; auto.
+     { case (eqbspec x z).
+       - intros ->; rewrite freevars_allvars; namedec.
+       - intros NE.
+         apply AEq_freevars in EQ.
+         rewrite (freevars_rename_subset3 v z), EQ.
+         rewrite freevars_rename_subset. namedec. }
+   + destruct IS1 as [->|(NI1,IS1)]; [easy|].
+     destruct IS2 as [->|(NI2,IS2)]; [easy|].
+     rewrite !mem_false by trivial.
+     set (vars :=
+            Names.add x (Names.add v (Names.add v'
+              (Names.unions
+                 [ Term.vars t; allvars f; allvars f'])))).
+     destruct (exist_fresh vars) as (z',Hz').
+     simpl_fresh vars Hz'.
+     apply AEq_rename_any with (z' := z') in EQ;
+       [ |namedec|namedec].
+     clear z H H0 H1.
+     apply AEqQu with z';
+       [rewrite 2 allvars_partialsubst; namedec|].
+     rewrite !rename_partialsubst in *; auto.
+     rewrite 2 (partialsubst_partialsubst x); auto;
+     try (rewrite !term_subst_notin by namedec);
+     try (apply IH; auto); cbn; try namedec;
+     try apply IsSimple_partialsubst; auto with set.
+     rewrite allvars_partialsubst. namedec.
+     rewrite allvars_partialsubst. namedec.
+Qed.
+
+Lemma AEq_SimpleSubst f1 f2 f1' f2' x t :
+ AlphaEq f1 f2 ->
+ SimpleSubst x t f1 f1' -> SimpleSubst x t f2 f2' ->
+ AlphaEq f1' f2'.
+Proof.
+ intros EQ S1 S2. rewrite SimpleSubst_carac in *.
+ destruct S1 as (<-,IS1).
+ destruct S2 as (<-,IS2).
+ apply AEq_partialsubst; auto.
+Qed.
+
+Lemma AEqQu_rename0 f q (v z : variable) :
+ IsSimple v z f -> ~Names.In z (freevars f) ->
+ AlphaEq (Quant q v f) (Quant q z (partialsubst v z f)).
+Proof.
+ intros IS NI.
+ set (vars := Names.add z (Names.add v (allvars f))).
+ destruct (exist_fresh vars) as (z',Hz').
+ apply AEqQu with z'.
+ - rewrite allvars_partialsubst. cbn. namedec.
+ - case (eqbspec v z).
+   + intros ->.
+     rewrite (partialsubst_notin z z); auto. reflexivity.
+   + intros NE.
+     rewrite !rename_partialsubst.
+     rewrite partialsubst_partialsubst; cbn; auto with set.
+     now rewrite eqb_refl, (partialsubst_notin z).
+     rewrite allvars_partialsubst. simpl. namedec. namedec.
+Qed.
+
+(** The full substitution, first as a relation *)
+
+Definition Subst x t f f' :=
+  exists f0, AlphaEq f f0 /\ SimpleSubst x t f0 f'.
+
+Lemma SimpleSubst_Subst x t f f' :
+  SimpleSubst x t f f' -> Subst x t f f'.
+Proof.
+ intros. now exists f.
+Qed.
+
+Lemma Subst_compat x t f1 f2 f1' f2' :
+ AlphaEq f1 f2 -> Subst x t f1 f1' -> Subst x t f2 f2' ->
+  AlphaEq f1' f2'.
+Proof.
+ intros EQ (f1b & EQ1 & S1) (f2b & EQ2 & S2).
+ apply (AEq_SimpleSubst f1b f2b f1' f2' x t); auto.
+ transitivity f1. now symmetry.
+ transitivity f2; auto.
+Qed.
+
+(* Pseudo constructors for Subst. *)
+
+Lemma Subst_True x t : Subst x t True True.
+Proof.
+ now apply SimpleSubst_Subst.
+Qed.
+
+Lemma Subst_False x t : Subst x t False False.
+Proof.
+ now apply SimpleSubst_Subst.
+Qed.
+
+Lemma Subst_Pred x t p l :
+  Subst x t (Pred p l) (partialsubst x t (Pred p l)).
+Proof.
+ apply SimpleSubst_Subst. now apply SimpleSubst_partialsubst.
+Qed.
+
+Lemma Subst_Not x t f f' :
+  Subst x t f f' -> Subst x t (~f) (~f').
+Proof.
+  intros (f0 & EQ & SI). exists (~ f0)%form; auto.
+Qed.
+
+Lemma Subst_Op x t o f1 f2 f1' f2' :
+  Subst x t f1 f1' -> Subst x t f2 f2' ->
+  Subst x t (Op o f1 f2) (Op o f1' f2').
+Proof.
+  intros (f1b & EQ1 & SI1) (f2b & EQ2 & SI2).
+  exists (Op o f1b f2b); auto.
+Qed.
+
+Lemma Subst_Qu1 x t q f :
+  Subst x t (Quant q x f) (Quant q x f).
+Proof.
+  exists (Quant q x f). split; auto. reflexivity.
+Qed.
+
+Lemma Subst_Qu2 x t q v f f' :
+  x <> v ->
+  ~Names.In v (Term.vars t) ->
+  Subst x t f f' ->
+  Subst x t (Quant q v f) (Quant q v f').
+Proof.
+  intros NE NI (f0 & EQ & IS).
+  exists (Quant q v f0). auto using AEqQu_nosubst.
+Qed.
+
+Lemma Subst_Qu3 x t q (v z : variable) f f' g :
+  x <> v ->
+  ~Names.In z (freevars f) ->
+  Subst v z f f' ->
+  Subst x t (Quant q z f') (Quant q z g) ->
+  Subst x t (Quant q v f) (Quant q z g).
+Proof.
+  intros NE NI (f0 & EQ & SI) (h & EQ' & SI').
+  exists h. split; auto.
+  transitivity (Quant q z f'); auto.
+  transitivity (Quant q v f0).
+  apply AEqQu_nosubst; auto.
+  rewrite SimpleSubst_carac in SI. destruct SI as (<-,IS).
+  apply AEqQu_rename0; auto.
+  apply AEq_freevars in EQ. now rewrite <- EQ.
+Qed.
+
+Lemma Subst_subst x t f : Subst x t f (subst x t f).
+Proof.
+ unfold subst.
+ set (h := S (height f)).
+ assert (LT : height f < h) by (cbn; auto with * ).
+ clearbody h. revert x t f LT.
+ induction h as [|h IH]; [inversion 1|];
+  intros x t [ ] LT; cbn -[fresh] in *; simpl_height.
+ - apply Subst_True.
+ - apply Subst_False.
+ - apply Subst_Pred.
+ - apply Subst_Not; auto.
+ - apply Subst_Op; auto.
+ - setfresh vars z Hz.
+   case eqbspec.
+   + intros ->. apply Subst_Qu1.
+   + intros NE.
+     destruct (Names.mem v (Term.vars t)) eqn:IN; cbn.
+     * clear IN.
+       apply Subst_Qu3 with (rename v z f); auto.
+       { rewrite freevars_allvars. namedec. }
+       { exists f. split. reflexivity.
+         rewrite rename_partialsubst by namedec.
+         apply SimpleSubst_partialsubst; auto with set. }
+       { apply Subst_Qu2; auto; try namedec. }
+     * apply Subst_Qu2; auto.
+       rewrite <- Names.mem_spec. now rewrite IN.
+Qed.
+
+Lemma Subst_exists x t f : exists f', Subst x t f f'.
+Proof.
+ exists (subst x t f). apply Subst_subst.
+Qed.
+
+Lemma Subst_compat' x t f1 f2 f1' :
+ AlphaEq f1 f2 -> Subst x t f1 f1' ->
+ exists f2', Subst x t f2 f2' /\ AlphaEq f1' f2'.
+Proof.
+ intros EQ SU.
+ exists (subst x t f2).
+ split. apply Subst_subst.
+ eapply Subst_compat; eauto. apply Subst_subst.
+Qed.
+
+Instance : Proper (eq ==> eq ==> AlphaEq ==> eq ==> iff) Subst.
+Proof.
+ intros x x' <- t t' <- f f' Hf g g' <-.
+ split.
+ - intros (f0 & EQ & SI).
+   exists f0. split; auto. now transitivity f.
+ - intros (f0 & EQ & SI).
+   exists f0. split; auto. now transitivity f'.
+Qed.
+
+Instance : Proper (eq ==> eq ==> AlphaEq ==> AlphaEq) subst.
+Proof.
+ intros x x' <- t t' <- f f' Hf.
+ apply (Subst_compat x t f f'); auto using Subst_subst.
+Qed.
+
+(** Substitution of a quantifier, general equation via a fresh
+    variable. *)
+
+Lemma subst_quant_gen q x v z t f :
+ x <> v ->
+ ~Names.In z (Names.add x (Names.union (allvars f) (Term.vars t))) ->
+ AlphaEq (subst x t (Quant q v f))
+         (Quant q z (subst x t (rename v z f))).
+Proof.
+ intros.
+ assert (AlphaEq (Quant q v f) (Quant q z (rename v z f))).
+ { apply AEqQu_rename. namedec. }
+ eapply Subst_compat; [apply H1|apply Subst_subst|].
+ apply Subst_Qu2.
+ - namedec.
+ - namedec.
+ - apply Subst_subst.
+Qed.
+
+(* TODO:
+    - faire sans partialsubst ?
+    - essayer une version simplifiée (sans Names.mem ...) *)
